\chapter{Symmetrization
and Antisymmetrization: COMING SOON}
\label{ch-sym}

$(1,2)$ transposition, swaps 1 and 2, $1\rarrow 2\rarrow 1$.
$(3,2,1)$ means $3\rarrow 2\rarrow 1\rarrow 3$. A
reordering of $(1,2,3,\ldots, p)$
is a permutation on $p$ letters.
A permutation can be expressed as a product of transpositions
 $(3,2,1)=(3,2)(2,1)$ is an
even permutation because
it can be expressed as a product of an even number of
transpositions. An odd permutation can be expressed as a product of an odd
number of permutations.

\section{Symmetrization}
\beq
\indi_{a_1,{a_2}}^{{b_2},{b_1}}
=
\delta_{a_1}^{b_1} \delta _{a_2}^{b_2}=
\bcen
\xymatrix@R=1pc@C=1pc{a_1
&{b_1}\ar[l]
\\
{a_2}
&{b_2}\ar[l]}
\ecen
\eeq

\beq
(\s_{(1,2)})_{a_1,{a_2}}^{{b_2},{b_1}}
=
\delta_{a_1}^{b_2} \delta _{a_2}^{b_1}=
\bcen
\xymatrix@R=1pc@C=1pc{a_1
&\bullet\ar@{<->}[d]\ar[l]
&{b_1}\ar[l]
\\
{a_2}
&\bullet \ar[l]
&{b_2}\ar[l]}
\ecen
\eeq

\beq
\indi =
\bcen
\xymatrix@R=1pc@C=1pc{
&&\ar[ll]
\\
&&\ar[ll]
\\
&&\ar[ll]
}
\ecen
\eeq

\beq
\s_{(1,2)} =
\bcen
\xymatrix@R=1pc@C=1pc{
&\bullet\ar@{<->}[d]
&\ar[ll]
\\
&\bullet
&\ar[ll]
\\
&&\ar[ll]
}
\ecen
\s_{(2,3)} =
\bcen
\xymatrix@R=1pc@C=1pc{
&
&\ar[ll]
\\
&\bullet\ar@{<->}[d]
\ar[l]
&\ar[l]
\\
&\bullet\ar[l]
&\ar[l]
}
\ecen
\s_{(1,3)} =
\bcen
\xymatrix@R=1pc@C=1pc{
&\bullet\ar@{<->}[dd]
&\ar[ll]
\\
&
&\ar[ll]
\\
&\bullet
&\ar[ll]
}
\ecen
\eeq

\beq
\s_{(1,2,3)} =
\bcen
\xymatrix@R=1pc@C=1pc{
&\bullet\ar@{<->}[d]\ar[l]
&
&\ar[ll]
\\
&\bullet
&\bullet\ar[ll]
\ar\ar@{<->}[d]
&\ar[l]
\\
&
&\bullet\ar[ll]
&\ar[l]
}
\ecen
=
\bcen
\xymatrix@R=1pc@C=1pc{
&
&\bullet\ar@{<->}[dd]\ar[ll]
&\ar[l]
\\
&\bullet\ar@{<->}[d]
\ar[l]
&
&\ar[ll]
\\
&\bullet\ar[l]
&\bullet\ar[l]
&\ar[l]
}
\ecen
\eeq

\beq
\s_{(1,3,2)} =
\bcen
\xymatrix@R=1pc@C=1pc{
&
&\bullet\ar@{<->}[d]\ar[ll]
&\ar[l]
\\
&\bullet\ar@{<->}[d]
\ar[l]
&\bullet\ar[l]
&\ar[l]
\\
&\bullet\ar[l]
&
&\ar[ll]
}
\ecen
=\bcen
\xymatrix@R=1pc@C=1pc{
&\bullet\ar@{<->}[d]\ar[l]
&\bullet\ar@{<->}[dd]
&\ar[ll]
\\
&\bullet\ar[l]
&
&\ar[ll]
\\
&
&\bullet\ar[ll]
&\ar[l]
}
\ecen
\eeq

\beq
\bcen
\xymatrix@R=1pc@C=1pc{
&\cals_p\ar@2{-}[dddd]\ar[l]
&\ar[l]
\\
&\ar[l]
&\ar[l]
\\
&\ar[l]
&\ar[l]
\\
\vdots&
&\vdots
\\
&\ar[l]
&\ar[l]
}
\ecen
=
\frac{1}{p!}
\left\{
\bcen
\xymatrix@R=1pc@C=1pc{
&
&\ar[ll]
\\
&
&\ar[ll]
\\
&
&\ar[ll]
\\
\vdots&
&\vdots
\\
&
&\ar[ll]
}
\ecen
+
\bcen
\xymatrix@R=1pc@C=1pc{
&\bullet\ar[l]
\ar@{<->}[d]
&\ar[l]
\\
&\bullet\ar[l]
&\ar[l]
\\
&
&\ar[ll]
\\
\vdots&
&\vdots
\\
&
&\ar[ll]
}
\ecen
+ \cdots
\right\}
\eeq


\beq
\cals^2_p = \cals_p
\eeq

\beq
\bcen
\xymatrix@R=1pc@C=1pc{
&\cals_p\ar@2{-}[dddd]\ar[l]
&\ar[l]
\\
&\ar[l]
&\ar[l]
\\
&\ar[l]
&\ar[l]
\\
\vdots&
&\vdots
\\
&\ar[l]
&\ar[l]
}\xymatrix@R=1pc@C=1pc{
&\cals_p\ar@2{-}[dddd]\ar[l]
&\ar[l]
\\
&\ar[l]
&\ar[l]
\\
&\ar[l]
&\ar[l]
\\
\vdots&
&\vdots
\\
&\ar[l]
&\ar[l]
}
\ecen
=
\bcen
\xymatrix@R=1pc@C=1pc{
&\cals_p\ar@2{-}[dddd]\ar[l]
&\ar[l]
\\
&\ar[l]
&\ar[l]
\\
&\ar[l]
&\ar[l]
\\
\vdots&
&\vdots
\\
&\ar[l]
&\ar[l]
}
\ecen
\eeq

\beq
\bcen
\xymatrix@R=1pc@C=1pc{
&\cals_p\ar@2{-}[dddd]\ar[l]
&\ar[l]
\\
&\ar[l]
&\ar[l]
\\
&\ar[l]
&\ar[l]
\\
\vdots&
&\vdots
\\
&\ar[l]
&\ar[l]
}\xymatrix@R=1pc@C=1pc{
&\cals_{[1,q]}\ar@2{-}[dd]\ar[l]
&\ar[l]
\\
&\ar[l]
&\ar[l]
\\
&\ar[l]
&\ar[l]
\\
\vdots&
&\vdots
\\
&
&\ar[ll]
}
\ecen
=
\bcen
\xymatrix@R=1pc@C=1pc{
&\cals_p\ar@2{-}[dddd]\ar[l]
&\ar[l]
\\
&\ar[l]
&\ar[l]
\\
&\ar[l]
&\ar[l]
\\
\vdots&
&\vdots
\\
&\ar[l]
&\ar[l]
}
\ecen
\eeq

\beq
\bcen
\xymatrix@R=1pc@C=1pc{
&\cals_p\ar@2{-}[dddd]\ar[l]
&\ar[l]
\\
&\ar[l]
&\ar[l]
\\
&\ar[l]
&\ar[l]
\\
\vdots&
&\vdots
\\
&\ar[l]
&\ar[l]
}\xymatrix@R=1pc@C=1pc{
&\bullet\ar@{<->}[d]\ar[l]
&\ar[l]
\\
&\bullet\ar[l]
&\ar[l]
\\
&\ar[l]
&\ar[l]
\\
\vdots&
&\vdots
\\
&
&\ar[ll]
}
\ecen
=
\bcen
\xymatrix@R=1pc@C=1pc{
&\cals_p\ar@2{-}[dddd]\ar[l]
&\ar[l]
\\
&\ar[l]
&\ar[l]
\\
&\ar[l]
&\ar[l]
\\
\vdots&
&\vdots
\\
&\ar[l]
&\ar[l]
}
\ecen
\eeq

\begin{claim}
\beq
\bcen
\xymatrix@R=1pc@C=1pc{
&\cals_p\ar@2{-}[dddd]\ar[l]
&\ar[l]
\\
&\ar[l]
&\ar[l]
\\
&\ar[l]
&\ar[l]
\\
\vdots&
&\vdots
\\
&\ar[l]
&\ar[l]
}
\ecen
=
\frac{1}{p}
\left(
\bcen
\xymatrix@R=1pc@C=1pc{
&
&\ar[ll]
\\
&\cals_{p-1}\ar@2{-}[ddd]\ar[l]
&\ar[l]
\\
&\ar[l]
&\ar[l]
\\
\vdots&
&\vdots
\\
&\ar[l]
&\ar[l]
}
\ecen
+
(p-1)
\bcen
\xymatrix@R=1pc@C=1pc{
&
&\bullet\ar[ll]\ar@{<->}[d]
&
&\ar[ll]
\\
&\cals_{p-1}\ar@2{-}[ddd]\ar[l]
&\bullet\ar[l]
&\cals_{p-1}\ar@2{-}[ddd]\ar[l]
&\ar[l]
\\
&\ar[l]
&&\ar[ll]
&\ar[l]
\\
\vdots&
&\vdots
&
&
\\
&\ar[l]
&
&\ar[ll]
&\ar[l]
}
\ecen
\right)
\eeq

\end{claim}
\proof
We only prove it for $p=3$.

\beq
3!
\bcen
\xymatrix@R=1pc@C=1pc{
&\cals_3\ar@2{-}[dd]\ar[l]
&\ar[l]
\\
&\ar[l]
&\ar[l]
\\
&\ar[l]
&\ar[l]
}
\ecen
=
\left(
\begin{array}{l}
\bcen
\xymatrix@R=1pc@C=1pc{
&&\ar[ll]
\\
&&\ar[ll]
\\
&&\ar[ll]
}
\ecen
+
\bcen
\xymatrix@R=1pc@C=1pc{
&\bullet\ar@{<->}[d]\ar[l]
&
&\ar[ll]
\\
&\bullet
&\bullet\ar[ll]
\ar\ar@{<->}[d]
&\ar[l]
\\
&
&\bullet\ar[ll]
&\ar[l]
}
\ecen
+
\bcen
\xymatrix@R=1pc@C=1pc{
&
&\bullet\ar@{<->}[d]\ar[ll]
&\ar[l]
\\
&\bullet\ar@{<->}[d]
\ar[l]
&\bullet\ar[l]
&\ar[l]
\\
&\bullet\ar[l]
&
&\ar[ll]
}
\ecen
\\
\\
+
\bcen
\xymatrix@R=1pc@C=1pc{
&
&\ar[ll]
\\
&\bullet\ar@{<->}[d]
\ar[l]
&\ar[l]
\\
&\bullet\ar[l]
&\ar[l]
}
\ecen
+
\bcen
\xymatrix@R=1pc@C=1pc{
&\bullet\ar@{<->}[d]
&\ar[ll]
\\
&\bullet
&\ar[ll]
\\
&&\ar[ll]
}
\ecen
+
\bcen
\xymatrix@R=1pc@C=1pc{
&\bullet\ar@{<->}[dd]
&\ar[ll]
\\
&
&\ar[ll]
\\
&\bullet
&\ar[ll]
}
\ecen
\end{array}
\right)
\eeq

\beq
2!
\bcen
\xymatrix@R=1pc@C=1pc{
&
&\ar[ll]
\\
&\cals_2\ar@2{-}[d]\ar[l]
&\ar[l]
\\
&\ar[l]
&\ar[l]
}
\ecen
=
\left(
\begin{array}{l}
\bcen
\xymatrix@R=1pc@C=1pc{
&&\ar[ll]
\\
&&\ar[ll]
\\
&&\ar[ll]
}
\ecen
+
\bcen
\xymatrix@R=1pc@C=1pc{
&
&\ar[ll]
\\
&\bullet\ar@{<->}[d]
\ar[l]
&\ar[l]
\\
&\bullet\ar[l]
&\ar[l]
}
\ecen
\end{array}
\right)
\eeq

\begin{align}
3!
\bcen
\xymatrix@R=1pc@C=1pc{
&\cals_3\ar@2{-}[dd]\ar[l]
&\ar[l]
\\
&\ar[l]
&\ar[l]
\\
&\ar[l]
&\ar[l]
}
\ecen
-
2!
\bcen
\xymatrix@R=1pc@C=1pc{
&
&\ar[ll]
\\
&\cals_2\ar@2{-}[d]\ar[l]
&\ar[l]
\\
&\ar[l]
&\ar[l]
}
\ecen
&=
\left(
\begin{array}{l}
\bcen
\xymatrix@R=1pc@C=1pc{
&\bullet\ar@{<->}[d]\ar[l]
&
&\ar[ll]
\\
&\bullet
&\bullet\ar[ll]
\ar\ar@{<->}[d]
&\ar[l]
\\
&
&\bullet\ar[ll]
&\ar[l]
}
\ecen
+
\bcen
\xymatrix@R=1pc@C=1pc{
&
&\bullet\ar@{<->}[d]\ar[ll]
&\ar[l]
\\
&\bullet\ar@{<->}[d]
\ar[l]
&\bullet\ar[l]
&\ar[l]
\\
&\bullet\ar[l]
&
&\ar[ll]
}
\ecen
\\
\\
+
\bcen
\xymatrix@R=1pc@C=1pc{
&\bullet\ar@{<->}[d]
&\ar[ll]
\\
&\bullet
&\ar[ll]
\\
&&\ar[ll]
}
\ecen
+
\bcen
\xymatrix@R=1pc@C=1pc{
&\bullet\ar@{<->}[dd]
&\ar[ll]
\\
&
&\ar[ll]
\\
&\bullet
&\ar[ll]
}
\ecen
\end{array}
\right)
\\
&=
2! 2!
\bcen
\xymatrix@R=1pc@C=1pc{
&
&\bullet\ar[ll]\ar@{<->}[d]
&
&\ar[ll]
\\
&\cals_{2}\ar@2{-}[d]\ar[l]
&\bullet\ar[l]
&\cals_{2}\ar@2{-}[d]\ar[l]
&\ar[l]
\\
&\ar[l]
&&\ar[ll]
&\ar[l]
}
\ecen
\end{align}
\qed

\begin{align}
\bcen
\xymatrix@R=1pc@C=1pc{
&\cals_p\ar@2{-}[dddd]\ar[l]
&\ar[l]
\ar@[red]@{-}@/_1pc/[ll]
\\
&\ar[l]
&\ar[l]
\\
&\ar[l]
&\ar[l]
\\
\vdots&
&\vdots
\\
&\ar[l]
&\ar[l]
}
\ecen
&=
\frac{1}{p}
\left(
\bcen
\xymatrix@R=1pc@C=1pc{
&
&\ar[ll]
\ar@[red]@{-}@/_1pc/[ll]
\\
&\cals_{p-1}\ar@2{-}[ddd]\ar[l]
&\ar[l]
\\
&\ar[l]
&\ar[l]
\\
\vdots&
&\vdots
\\
&\ar[l]
&\ar[l]
}
\ecen
+
(p-1)
\bcen
\xymatrix@R=1pc@C=1pc{
&
&\bullet\ar[ll]\ar@{<->}[d]
&
&\ar[ll]
\ar@[red]@{-}@/_1pc/[llll]
\\
&\cals_{p-1}\ar@2{-}[ddd]\ar[l]
&\bullet\ar[l]
&\cals_{p-1}\ar@2{-}[ddd]\ar[l]
&\ar[l]
\\
&\ar[l]
&&\ar[ll]
&\ar[l]
\\
\vdots&
&\vdots
&
&
\\
&\ar[l]
&
&\ar[ll]
&\ar[l]
}
\ecen
\right)
\\
&=
\frac{n+p-1}{p}
\left(
\bcen
\xymatrix@R=1pc@C=1pc{
&\cals_{p-1}\ar@2{-}[ddd]\ar[l]
&\ar[l]
\\
&\ar[l]
&\ar[l]
\\
\vdots&
&\vdots
\\
&\ar[l]
&\ar[l]
}
\ecen
\right)
\end{align}


\beq
\tr_{\rva_1}\cals_p = \frac{n+p-1}{p}\cals_{p-1}
\eeq

\beq
\tr_{\rva_1, \rva_2, \ldots, \rva_k}\cals_p = \frac{(n+p-1)(n+p-2)\ldots
(n=p-k)}
{p(p-1)\ldots(p-k+1)}
\cals_{p-k}
\eeq

\beq
d_{\cals_p}=
\tr_{\rva^p}\cals_p=
\frac{(n+p-1)!}{p!(n-1)!}=
{n+p-1\choose p}
\eeq
For $p=2$, 

\beq
d_{\cals_2}=
\frac{(n+1)n}{2}
\eeq

\section{Antisymmetrization}

\beq
\bcen
\xymatrix@R=1pc@C=1pc{
&\cala_p\ar@2{-}[dddd]\ar[l]
&\ar[l]
\\
&\ar[l]
&\ar[l]
\\
&\ar[l]
&\ar[l]
\\
\vdots&
&\vdots
\\
&\ar[l]
&\ar[l]
}
\ecen
=
\frac{1}{p!}
\left\{
\bcen
\xymatrix@R=1pc@C=1pc{
&
&\ar[ll]
\\
&
&\ar[ll]
\\
&
&\ar[ll]
\\
\vdots&
&\vdots
\\
&
&\ar[ll]
}
\ecen
-
\bcen
\xymatrix@R=1pc@C=1pc{
&\bullet\ar[l]
\ar@{<->}[d]
&\ar[l]
\\
&\bullet\ar[l]
&\ar[l]
\\
&
&\ar[ll]
\\
\vdots&
&\vdots
\\
&
&\ar[ll]
}
\ecen
+ \cdots
\right\}
\eeq

\beq
\cala^2_p = \cala_p
\eeq

\beq
\bcen
\xymatrix@R=1pc@C=1pc{
&\cala_p\ar@2{-}[dddd]\ar[l]
&\ar[l]
\\
&\ar[l]
&\ar[l]
\\
&\ar[l]
&\ar[l]
\\
\vdots&
&\vdots
\\
&\ar[l]
&\ar[l]
}\xymatrix@R=1pc@C=1pc{
&\cala_p\ar@2{-}[dddd]\ar[l]
&\ar[l]
\\
&\ar[l]
&\ar[l]
\\
&\ar[l]
&\ar[l]
\\
\vdots&
&\vdots
\\
&\ar[l]
&\ar[l]
}
\ecen
=
\bcen
\xymatrix@R=1pc@C=1pc{
&\cala_p\ar@2{-}[dddd]\ar[l]
&\ar[l]
\\
&\ar[l]
&\ar[l]
\\
&\ar[l]
&\ar[l]
\\
\vdots&
&\vdots
\\
&\ar[l]
&\ar[l]
}
\ecen
\eeq

\beq
\bcen
\xymatrix@R=1pc@C=1pc{
&\cala_p\ar@2{-}[dddd]\ar[l]
&\ar[l]
\\
&\ar[l]
&\ar[l]
\\
&\ar[l]
&\ar[l]
\\
\vdots&
&\vdots
\\
&\ar[l]
&\ar[l]
}\xymatrix@R=1pc@C=1pc{
&\cala_{[1,q]}\ar@2{-}[dd]\ar[l]
&\ar[l]
\\
&\ar[l]
&\ar[l]
\\
&\ar[l]
&\ar[l]
\\
\vdots&
&\vdots
\\
&
&\ar[ll]
}
\ecen
=
\bcen
\xymatrix@R=1pc@C=1pc{
&\cala_p\ar@2{-}[dddd]\ar[l]
&\ar[l]
\\
&\ar[l]
&\ar[l]
\\
&\ar[l]
&\ar[l]
\\
\vdots&
&\vdots
\\
&\ar[l]
&\ar[l]
}
\ecen
\eeq

\beq
\bcen
\xymatrix@R=1pc@C=1pc{
&\cala_p\ar@2{-}[dddd]\ar[l]
&\ar[l]
\\
&\ar[l]
&\ar[l]
\\
&\ar[l]
&\ar[l]
\\
\vdots&
&\vdots
\\
&\ar[l]
&\ar[l]
}\xymatrix@R=1pc@C=1pc{
&\bullet\ar@{<->}[d]\ar[l]
&\ar[l]
\\
&\bullet\ar[l]
&\ar[l]
\\
&\ar[l]
&\ar[l]
\\
\vdots&
&\vdots
\\
&
&\ar[ll]
}
\ecen
= (-1)
\bcen
\xymatrix@R=1pc@C=1pc{
&\cala_p\ar@2{-}[dddd]\ar[l]
&\ar[l]
\\
&\ar[l]
&\ar[l]
\\
&\ar[l]
&\ar[l]
\\
\vdots&
&\vdots
\\
&\ar[l]
&\ar[l]
}
\ecen
\eeq

\beq
\cals_p\cala_q = \cala_p\cals_q=0
\eeq

\beq
\bcen
\xymatrix@R=1pc@C=1pc{
&\cals_p\ar@2{-}[dddd]\ar[l]
&\ar[l]
\\
&\ar[l]
&\ar[l]
\\
&\ar[l]
&\ar[l]
\\
\vdots&
&\vdots
\\
&\ar[l]
&\ar[l]
}\xymatrix@R=1pc@C=1pc{
&\cala_p\ar@2{-}[dddd]\ar[l]
&\ar[l]
\\
&\ar[l]
&\ar[l]
\\
&\ar[l]
&\ar[l]
\\
\vdots&
&\vdots
\\
&\ar[l]
&\ar[l]
}
\ecen
=0
\eeq

\beq
\bcen
\xymatrix@R=1pc@C=1pc{
&\cals_p\ar@2{-}[dddd]\ar[l]
&\ar[l]
\\
&\ar[l]
&\ar[l]
\\
&\ar[l]
&\ar[l]
\\
\vdots&
&\vdots
\\
&\ar[l]
&\ar[l]
}\xymatrix@R=1pc@C=1pc{
&\cala_{[1,q]}\ar@2{-}[dd]\ar[l]
&\ar[l]
\\
&\ar[l]
&\ar[l]
\\
&\ar[l]
&\ar[l]
\\
\vdots&
&\vdots
\\
&
&\ar[ll]
}
\ecen
=
\bcen
\xymatrix@R=1pc@C=1pc{
&\cala_p\ar@2{-}[dddd]\ar[l]
&\ar[l]
\\
&\ar[l]
&\ar[l]
\\
&\ar[l]
&\ar[l]
\\
\vdots&
&\vdots
\\
&\ar[l]
&\ar[l]
}\xymatrix@R=1pc@C=1pc{
&\cals_{[1,q]}\ar@2{-}[dd]\ar[l]
&\ar[l]
\\
&\ar[l]
&\ar[l]
\\
&\ar[l]
&\ar[l]
\\
\vdots&
&\vdots
\\
&
&\ar[ll]
}
\ecen
=
0
\eeq

\begin{claim}
\beq
\bcen
\xymatrix@R=1pc@C=1pc{
&\cala_p\ar@2{-}[dddd]\ar[l]
&\ar[l]
\\
&\ar[l]
&\ar[l]
\\
&\ar[l]
&\ar[l]
\\
\vdots&
&\vdots
\\
&\ar[l]
&\ar[l]
}
\ecen
=
\frac{1}{p}
\left(
\bcen
\xymatrix@R=1pc@C=1pc{
&
&\ar[ll]
\\
&\cala_{p-1}\ar@2{-}[ddd]\ar[l]
&\ar[l]
\\
&\ar[l]
&\ar[l]
\\
\vdots&
&\vdots
\\
&\ar[l]
&\ar[l]
}
\ecen
+
{\color{red}(-1)}(p-1)
\bcen
\xymatrix@R=1pc@C=1pc{
&
&\bullet\ar[ll]\ar@{<->}[d]
&
&\ar[ll]
\\
&\cala_{p-1}\ar@2{-}[ddd]\ar[l]
&\bullet\ar[l]
&\cala_{p-1}\ar@2{-}[ddd]\ar[l]
&\ar[l]
\\
&\ar[l]
&&\ar[ll]
&\ar[l]
\\
\vdots&
&\vdots
&
&
\\
&\ar[l]
&
&\ar[ll]
&\ar[l]
}
\ecen
\right)
\eeq

\end{claim}
\proof
We only prove it for $p=3$.

\beq
3!
\bcen
\xymatrix@R=1pc@C=1pc{
&\cala_3\ar@2{-}[dd]\ar[l]
&\ar[l]
\\
&\ar[l]
&\ar[l]
\\
&\ar[l]
&\ar[l]
}
\ecen
=
\left(
\begin{array}{l}
\bcen
\xymatrix@R=1pc@C=1pc{
&&\ar[ll]
\\
&&\ar[ll]
\\
&&\ar[ll]
}
\ecen
+
\bcen
\xymatrix@R=1pc@C=1pc{
&\bullet\ar@{<->}[d]\ar[l]
&
&\ar[ll]
\\
&\bullet
&\bullet\ar[ll]
\ar\ar@{<->}[d]
&\ar[l]
\\
&
&\bullet\ar[ll]
&\ar[l]
}
\ecen
+
\bcen
\xymatrix@R=1pc@C=1pc{
&
&\bullet\ar@{<->}[d]\ar[ll]
&\ar[l]
\\
&\bullet\ar@{<->}[d]
\ar[l]
&\bullet\ar[l]
&\ar[l]
\\
&\bullet\ar[l]
&
&\ar[ll]
}
\ecen
\\
\\
-
\bcen
\xymatrix@R=1pc@C=1pc{
&
&\ar[ll]
\\
&\bullet\ar@{<->}[d]
\ar[l]
&\ar[l]
\\
&\bullet\ar[l]
&\ar[l]
}
\ecen
-
\bcen
\xymatrix@R=1pc@C=1pc{
&\bullet\ar@{<->}[d]
&\ar[ll]
\\
&\bullet
&\ar[ll]
\\
&&\ar[ll]
}
\ecen
-
\bcen
\xymatrix@R=1pc@C=1pc{
&\bullet\ar@{<->}[dd]
&\ar[ll]
\\
&
&\ar[ll]
\\
&\bullet
&\ar[ll]
}
\ecen
\end{array}
\right)
\eeq

\beq
2!
\bcen
\xymatrix@R=1pc@C=1pc{
&
&\ar[ll]
\\
&\cala_2\ar@2{-}[d]\ar[l]
&\ar[l]
\\
&\ar[l]
&\ar[l]
}
\ecen
=
\left(
\begin{array}{l}
\bcen
\xymatrix@R=1pc@C=1pc{
&&\ar[ll]
\\
&&\ar[ll]
\\
&&\ar[ll]
}
\ecen
-
\bcen
\xymatrix@R=1pc@C=1pc{
&
&\ar[ll]
\\
&\bullet\ar@{<->}[d]
\ar[l]
&\ar[l]
\\
&\bullet\ar[l]
&\ar[l]
}
\ecen
\end{array}
\right)
\eeq

\begin{align}
3!
\bcen
\xymatrix@R=1pc@C=1pc{
&\cala_3\ar@2{-}[dd]\ar[l]
&\ar[l]
\\
&\ar[l]
&\ar[l]
\\
&\ar[l]
&\ar[l]
}
\ecen
-
2!
\bcen
\xymatrix@R=1pc@C=1pc{
&
&\ar[ll]
\\
&\cala_2\ar@2{-}[d]\ar[l]
&\ar[l]
\\
&\ar[l]
&\ar[l]
}
\ecen
&=
\left(
\begin{array}{l}
\bcen
\xymatrix@R=1pc@C=1pc{
&\bullet\ar@{<->}[d]\ar[l]
&
&\ar[ll]
\\
&\bullet
&\bullet\ar[ll]
\ar\ar@{<->}[d]
&\ar[l]
\\
&
&\bullet\ar[ll]
&\ar[l]
}
\ecen
+
\bcen
\xymatrix@R=1pc@C=1pc{
&
&\bullet\ar@{<->}[d]\ar[ll]
&\ar[l]
\\
&\bullet\ar@{<->}[d]
\ar[l]
&\bullet\ar[l]
&\ar[l]
\\
&\bullet\ar[l]
&
&\ar[ll]
}
\ecen
\\
\\
-
\bcen
\xymatrix@R=1pc@C=1pc{
&\bullet\ar@{<->}[d]
&\ar[ll]
\\
&\bullet
&\ar[ll]
\\
&&\ar[ll]
}
\ecen
-
\bcen
\xymatrix@R=1pc@C=1pc{
&\bullet\ar@{<->}[dd]
&\ar[ll]
\\
&
&\ar[ll]
\\
&\bullet
&\ar[ll]
}
\ecen
\end{array}
\right)
\\
&=
{\color{red}(-1)}2! 2!
\bcen
\xymatrix@R=1pc@C=1pc{
&
&\bullet\ar[ll]\ar@{<->}[d]
&
&\ar[ll]
\\
&\cala_{2}\ar@2{-}[d]\ar[l]
&\bullet\ar[l]
&\cala_{2}\ar@2{-}[d]\ar[l]
&\ar[l]
\\
&\ar[l]
&&\ar[ll]
&\ar[l]
}
\ecen
\end{align}
\qed

\begin{align}
\bcen
\xymatrix@R=1pc@C=1pc{
&\cala_p\ar@2{-}[dddd]\ar[l]
&\ar[l]
\ar@[red]@{-}@/_1pc/[ll]
\\
&\ar[l]
&\ar[l]
\\
&\ar[l]
&\ar[l]
\\
\vdots&
&\vdots
\\
&\ar[l]
&\ar[l]
}
\ecen
&=
\frac{1}{p}
\left(
\bcen
\xymatrix@R=1pc@C=1pc{
&
&\ar[ll]
\ar@[red]@{-}@/_1pc/[ll]
\\
&\cala_{p-1}\ar@2{-}[ddd]\ar[l]
&\ar[l]
\\
&\ar[l]
&\ar[l]
\\
\vdots&
&\vdots
\\
&\ar[l]
&\ar[l]
}
\ecen
+{\color{red}(-1)}
(p-1)
\bcen
\xymatrix@R=1pc@C=1pc{
&
&\bullet\ar[ll]\ar@{<->}[d]
&
&\ar[ll]
\ar@[red]@{-}@/_1pc/[llll]
\\
&\cala_{p-1}\ar@2{-}[ddd]\ar[l]
&\bullet\ar[l]
&\cala_{p-1}\ar@2{-}[ddd]\ar[l]
&\ar[l]
\\
&\ar[l]
&&\ar[ll]
&\ar[l]
\\
\vdots&
&\vdots
&
&
\\
&\ar[l]
&
&\ar[ll]
&\ar[l]
}
\ecen
\right)
\\
&=
\frac{n+{\color{red}(-1)}(p-1)}{p}
\left(
\bcen
\xymatrix@R=1pc@C=1pc{
&\cala_{p-1}\ar@2{-}[ddd]\ar[l]
&\ar[l]
\\
&\ar[l]
&\ar[l]
\\
\vdots&
&\vdots
\\
&\ar[l]
&\ar[l]
}
\ecen
\right)
\end{align}

\beq
\tr_{\rva_1}\cala_p = \frac{n-p+1}{p}\cala_{p-1}
\eeq

\beq
\tr_{\rva_1, \rva_2, \ldots, \rva_k}\cala_p = \frac{(n-p+1)(n-p+2)\ldots
(n-p+k)}
{p(p-1)\ldots(p-k+1)}
\cala_{p-k}
\eeq

\beqa
d_{\cala_p}=
\tr_{\rva^p}\cala_p
&=&
\frac{\prod_{i=n-p+1}^n i}{p!}
\\
&=&
\frac{\prod
^{n-p+1}_{i=n} i}{p!}
\\
&=&
\left\{
\begin{array}{ll}
\frac{n!}{p!(n-p)!}={n\choose p} & 
\text{if } p\leq n
\\
0 & \text{otherwise}
\end{array}
\right.
\eeqa
For $p=2\leq n$, 

\beq
d_{\cala_2}=
{n\choose 2}
\eeq

\beq
\cala_p = 0
\text{ if } n < p
\eeq
For example, for $n=2$ and $p=3$

\beq
\bcen
\xymatrix@C=.3pc@R=1.5pc{
\ket{a}\ar[d]
&\ket{a}\ar[d]
&\ket{b}\ar[d]
\\
\cala_3\ar@2{-}[rr]
\ar[d]
&\ar[d]
&\ar[d]
\\
&&
}
\ecen
=
\frac{1}{6}
\left(
\begin{array}{l}
\bcen
\xymatrix@C=.3pc@R=1.5pc{
\ket{a}\ar[dd]
&\ket{a}\ar[dd]
&\ket{b}\ar[dd]
\\
&
&
\\
&&&
}
\ecen
+
\bcen
\xymatrix@C=.3pc@R=1.5pc{
\ket{a}\ar[d]
&\ket{a}\ar[d]
&\ket{b}\ar[dd]
\\
\bullet\ar[dd]\ar@{<->}[r]
&\bullet\ar[d]
&
\\
&\bullet\ar[d]\ar@{<->}[r]
&\bullet\ar[d]
\\
&&
}
\ecen
+\bcen
\xymatrix@C=.3pc@R=1.5pc{
\ket{a}\ar[dd]
&\ket{a}\ar[d]
&\ket{b}\ar[d]
\\
&\bullet\ar[d]\ar@{<->}[r]
&\bullet\ar[dd]
\\
\bullet\ar[d]\ar@{<->}[r]
&\bullet\ar[d]
&
\\
&&
}
\ecen
\\
\\
-
\bcen
\xymatrix@C=.3pc@R=1.5pc{
\ket{a}\ar[dd]
&\ket{a}\ar[d]
&\ket{b}\ar[d]
\\
\ar[d]
&\bullet\ar@{<->}[r]\ar[]
&\bullet\ar[d]
\\
&&&
}
\ecen
-
\bcen
\xymatrix@C=.3pc@R=1.5pc{
\ket{a}\ar[d]
&\ket{a}\ar[d]
&\ket{b}\ar[dd]
\\
\bullet\ar[d]\ar@{<->}[r]
&\bullet\ar[d]
&
\\
&&
}
\ecen
-
\bcen
\xymatrix@C=.3pc@R=1.5pc{
\ket{a}\ar[d]
&\ket{a}\ar[dd]
&\ket{b}\ar[d]
\\
\bullet\ar@{<->}[rr]
\ar[d]
&
&\bullet\ar[d]
\\
&&
}
\ecen
\end{array}
\right)
\eeq

\beqa
\cala_3\ket{a,a,b}&=&
\frac{1}{6}
\left(
\begin{array}{l}
\ket{a,a,b} + \ket{a,b,a} + \ket{b,a,a}
\\
-\ket{a,b,a} -\ket{a,a,b} - \ket{b,a,a}
\end{array}
\right)
\\
&=& 0
\eeqa





