\chapter{Spinors}
\label{ch-spinors}



This chapter is based on Cvitanovic's Birdtracks book Ref. \cite{birdtracks-book}.

The reader should read 
Chapter \ref{ch-paulions}
before reading this chapter. There he
will learn about
the group $Spin(n)_\RR$.


Let
\beq
\gamma_{\mu\nu}=\frac{1}{2}
[\gamma_\mu, \gamma_\nu]
\eeq


If $\gamma_\mu^\dagger=\gamma_\mu$
for $\mu=1,2,\ldots,n$ (this assumes the Euclidean metric which is  $g_{\mu\nu}=diag(1, 1, 1, 1)$ for $n=4$)
\beq
Spin(n)_\RR=
\{e^{\omega^{\mu\nu}\gamma_{\mu\nu}}|
\omega_{\mu\nu}=-\omega_{\nu\mu}\in\RR\}
\}
\eeq
If $\gamma_0^\dagger=\gamma_0$, and
$\gamma_i^\dagger=-\gamma_i$ (this assumes the mostly-minus metric which is $g_{\mu\nu}=diag(1, -1, -1, -1)$ for $n=4$)
\beq
Spin(1,3)_\RR=
\{e^{-i\omega^{\mu\nu}\gamma_{\mu\nu}}|
\omega_{\mu\nu}=-\omega_{\nu\mu},
\omega_{0,i}\in\RR, \omega_{i,j}
\in i\RR
\}
\eeq

{\bf Spinors} are the vectors in the vector space
upon which the group $Spin(n)_\RR$ acts.

\begin{table}[h!]
\begin{tabular}{|
>{\columncolor[HTML]{FFFFC7}}l |l|l|l|l|l|l|l|l|l|l|}
\hline
$n$ & 1 & 2 & 3 & 4 & 5 & 6 & 7 & 8 & 9 & 10 \\ \hline
$\intntwo$ & 0 & 1 & 1 & 2 & 2 & 3 & 3 & 4 & 4 & 5 \\ \hline
$d=2^{\intntwo}$ & 1 & 2 & 2 & 4 & 4 & 8 & 8 & 16 & 16 & 32 \\ \hline
\end{tabular}
\caption{$\gamma_\mu \in \CC^{d\times d}$}
\label{tab2-gamma-dim}
\end{table}


Let 
$
\mu \in \{1,2, \dots, n\}$


$int(x) =$ integer part of $x\in \RR$

$a,b\in\{ 1, 2, \ldots, 2^\intntwo\}$

$\gamma_\mu\in \CC^{d\times d}$ where 
$d=2^{int(n/2)}$ (See Table \ref{tab2-gamma-dim})

Define the following birdtracks
\beq
\gamma^\mu_{ab}
=
\bcen
\xymatrix{
&\mu\ar[d]
\\
a&
\ol{\gamma}
\ar@{-->}[l]
&b\ar@{-->}[l]
}
\ecen
,\quad
(\gamma_\mu)_{ab}
=
\bcen
\xymatrix{
&\mu
\\
a&
\ul{\gamma}\ar[u]
\ar@{-->}[l]
&b\ar@{-->}[l]
}
\ecen
,\quad
\delta_a^b=
\xymatrix{a
&\bullet&\ar@{-->}[ll]
}b
\eeq

\beq
g_{\mu\nu}= \xymatrix{\mu&\ul{g}\ar[r]\ar[l]&\nu},
\quad
g^{\mu\nu}= \xymatrix{\mu\ar[r]&\ol{g}&\ar[l]\nu}
\eeq

Note that



\beq
g\indices{_\mu^\mu}=
\dashbubble
=
2^{\intntwo}
\eeq

Clifford Algebra anticommutator:

\beq
\begin{array}{ll}
\myboxed{g_{\mu, \nu}\indi=\frac{1}{2}[\gamma_\mu, \gamma_\nu]_+}
&
\\
\bcen
\xymatrix{
&
\ar@{-}@/_2pc/[r]|{\ul{g}}
&
&
\\
\\
&&&\ar@{-->}[lll]
}
\ecen
&=
\bcen
\xymatrix{
&
& 
\\ 
&\cals_2\ar@2{-}[r]\ar[u]
&\ar[u]
&
\\
&\ar[u]\ul{\gamma}\ar@{-->}[l]
&\ar[u]\ul{\gamma} \ar@{-->}[l]
&\ar@{-->}[l]
}
\ecen
\\
&=
\frac{1}{2}
\left[
\bcen
\xymatrix{ 
&
&
&
\\
&\ul{\gamma}\ar@{-->}[l]\ar[u]
&\ul{\gamma} \ar@{-->}[l]\ar[u]
&\ar@{-->}[l]
}
\ecen
+
\bcen
\xymatrix{ 
&
&
&
\\
&\ul{\gamma}\ar@{-->}[l]\ar[ur]
&\ul{\gamma} \ar@{-->}[l]\ar[ul]
&\ar@{-->}[l]
}
\ecen
\right]
\end{array}
\label{eq-g-anti-com}
\eeq

By virtue of Eq.(\ref{eq-g-anti-com}),
it is possible to replace all $g$'s by swaps, 
and vice versa,
in a linear combination of birdtracks.

\begin{claim} 

\beq
\bcen
\xymatrix{
&\ar@{-->}[l]\ul{\gamma}
&\ar@{-}@/_2pc/[l]|{\ol{g}}
\ar@{-->}[l]\ul{\gamma}
&\ar@{-->}[l]
}
\ecen
=
n
\bcen
\xymatrix{
&&
&\ar@{-->}[lll]
}
\ecen
\eeq
\end{claim}
\proof
\beq
\bcen
\xymatrix{
&
&\ar@{-}@/_1pc/[l]|{\ol{g}}
\\ 
&\cals_2\ar@2{-}[r]\ar[u]
&\ar[u]
&
\\
&\ar[u]\ul{\gamma}\ar@{-->}[l]
&\ar[u]\ul{\gamma} \ar@{-->}[l]
&\ar@{-->}[l]
}
\ecen
=
\bcen
\xymatrix{
&
\ar@{-}@/_2pc/[r]|{\ul{g}}
&\ar@{-}@/_1pc/[l]|{\ol{g}}
&
\\
\\
&&&\ar@{-->}[lll]
}
\ecen
\eeq
\qed

\begin{claim}
\beq
\bcen
\xymatrix@C=1pc@R=1.5pc{
&&&&
\\
\cala_p\ar@2{-}[rrr]
\ar[u]
&\ar[u]
&\ar[u]
&\ar[u]
\\
\ar[u]
\ul{\gamma}
&\ar[u]\ar@{-->}[l]\ul{\gamma}
&\ar[u]\ar@{-->}[l]\ul{\gamma}
&\ar[u]\ar@{-->}[l]\ul{\gamma}
}
\ecen
=
\bcen
\xymatrix@C=1pc@R=1.5pc{
&&&
\\
&\cala_{p-1}\ar@2{-}[rr]\ar[u]
&\ar[u]
&\ar[u]
\\
\ul{\gamma}\ar[uu]
&\ar[u]\ar@{-->}[l]\ul{\gamma}
&\ar[u]\ar@{-->}[l]\ul{\gamma}
&\ar[u]\ar@{-->}[l]\ul{\gamma}
}
\ecen
-(p-1)
\bcen
\xymatrix@C=1pc@R=1.5pc{
%\ar@{-}`d[ddr]`[rd][rd]
&&&
\\
\ar@{-}@/_1pc/[r]|{\ul{g}}
&\cala_{p-1}\ar@2{-}[rr]\ar[u]
&\ar[u]
&\ar[u]
\\
&
&\ar@{-->}[ll]\ul{\gamma}\ar[u]
&\ar[u]
\ar@{-->}[l]\ul{\gamma}
}
\ecen
\eeq
\proof
\end{claim}

The claim for $p=2$ is
\beq
\bcen
\xymatrix@C=1pc@R=1.5pc{
&
\\
\cala_2\ar@2{-}[r]
\ar[u]
&\ar[u]
\\
\ar[u]\ul{\gamma}
&\ar[u]
\ar@{-->}[l]
\ul{\gamma}
}
\ecen
=
\bcen
\xymatrix@C=1pc@R=1.5pc{
&
\\
&
\\
\ul{\gamma}\ar[uu]
&\ar@{-->}[l]
\ul{\gamma}\ar[uu]
}
\ecen
-
\bcen
\xymatrix@C=2pc{
%\ar@{-}`d[ddr]`[r][r]
\ar@{-}@/_1pc/[r]|{\ul{g}}
&
\\
&
\\
&\ar@{-->}[l]
}
\ecen
\eeq
where we define

\beq
2
\bcen
\xymatrix@C=1pc@R=1.5pc{
&
\\
\cala_2\ar@2{-}[r]\ar[u]
&\ar[u]
\\
\ar[u]\ul{\gamma}
&\ar[u]
\ar@{-->}[l]
\ul{\gamma}
}
\ecen
=
\bcen
\xymatrix@C=1pc@R=1.5pc{
&
\\
&
\\
\ul{\gamma}\ar[uu]
&\ar@{-->}[l]
\ul{\gamma}\ar[uu]
}
\ecen
-
\bcen
\xymatrix@C=1pc@R=1.5pc{
&
\\
\ar@{<->}[r]\ar[u]
&\ar[u]
\\
\ar[u]\ul{\gamma}
&\ar[u]
\ar@{-->}[l]
\ul{\gamma}
}
\ecen
\eeq


The claim for $p=3$ is
\begin{align}
\bcen
\xymatrix@C=1pc@R=1.5pc{
&&
\\
\cala_3\ar@2{-}[rr]\ar[u]
&\ar[u]
&\ar[u]
\\
\ar[u]\ul{\gamma}
&\ar[u]\ul{\gamma}\ar@{-->}[l]
&\ar[u]\ul{\gamma}
\ar@{-->}[l]
}
\ecen
&=
\bcen
\xymatrix@C=1pc@R=1.5pc{
&&
\\
&\cala_{2}\ar@2{-}[r]\ar[u]
&\ar[u]
\\
\ul{\gamma}\ar[uu]
&\ar[u]\ul{\gamma}
\ar@{-->}[l]
&\ar[u]\ul{\gamma}
\ar@{-->}[l]
}
\ecen
-2
\bcen
\xymatrix@C=1pc@R=1.5pc{
%\ar@{-}`d[ddr]`[rd][rd]
&&
\\
\ar@{-}@/_1pc/[r]|{\ul{g}}
&\cala_{2}\ar@2{-}[r]\ar[u]
&\ar[u]
\\
&
&\ar[u]
\ar@{-->}[ll]
\ul{\gamma}
}
\ecen
\\
&=
\left[
\begin{array}{ll}
\bcen
\xymatrix@C=1pc@R=1.5pc{
&&
\\
&&
\\
\ul{\gamma}\ar[uu]
&\ul{\gamma}\ar[uu]\ar@{-->}[l]
&\ul{\gamma}\ar[uu]
\ar@{-->}[l]
}
\ecen
-
\bcen
\xymatrix@C=1pc@R=1.5pc{
&%\ar@{-}`d[ddr]`[r][r]
\ar@{-}@/_1pc/[r]|{\ul{g}}
&
\\
&
&
\\
\ul{\gamma}\ar[uu]
&
&\ar@{-->}[ll]
}
\ecen
\\
-
\bcen
\xymatrix@C=1pc@R=1.5pc{
%\ar@{-}`d[ddr]`[r][r]
\ar@{-}@/_1pc/[r]|{\ul{g}}
&
&
\\
&
&
\\
&
&
\ar@{-->}[ll]
\ul{\gamma}\ar[uu]
}
\ecen
+
\bcen
\xymatrix@C=1pc@R=1.5pc{
%\ar@{-}`d[ddr]`[r][r]
\ar@{-}@/_1.5pc/[rr]|{\ul{g}}
&
&
\\
&
&
\\
&\ul{\gamma}\ar@{-->}[l]\ar[uu]
&
\ar@{-->}[l]
}
\ecen
\end{array}
\right]
\end{align}
where we define

\beq
6
\bcen
\xymatrix@C=1pc@R=1.5pc{
&&
\\
\cala_3\ar@2{-}[rr]\ar[u]
&\ar[u]
&\ar[u]
\\
\ar[u]\ul{\gamma}
&\ar[u]\ul{\gamma}\ar@{-->}[l]
&\ar[u]\ul{\gamma}
\ar@{-->}[l]
}
\ecen
=
\left[
\begin{array}{ll}
\bcen
\xymatrix@C=1pc@R=1.5pc{
&&
\\
&&
\\
\ul{\gamma}\ar[uu]
&\ul{\gamma}\ar[uu]\ar@{-->}[l]
&\ul{\gamma}\ar[uu]
\ar@{-->}[l]
}
\ecen
-
\bcen
\xymatrix@C=1pc@R=1.5pc{
&&
\\
\ar@{<->}[r]
&
&
\\
\ul{\gamma}\ar[uu]
&\ul{\gamma}\ar@{-->}[l]\ar[uu]
&\ul{\gamma}\ar[uu]
\ar@{-->}[l]
}
\ecen
-
\bcen
\xymatrix@C=1pc@R=1.5pc{
&&
\\
&\ar@{<->}[r]
&
\\
\ul{\gamma}\ar[uu]
&\ul{\gamma}\ar@{-->}[l]\ar[uu]
&\ul{\gamma}\ar[uu]
\ar@{-->}[l]
}
\ecen
\\
-
\bcen
\xymatrix@C=1pc@R=1.5pc{
&&
\\
\ar@{<->}[rr]&&
\\
\ul{\gamma}\ar[uu]
&\ul{\gamma}\ar@{-->}[l]\ar[uu]
&\ul{\gamma}\ar[uu]
\ar@{-->}[l]
}
\ecen
+
\bcen
\xymatrix@C=1pc@R=1.5pc{
&&
\\
&\ar@{<->}[r]
&
\\
\ar@{<->}[r]
&&
\\
\ul{\gamma}\ar[uuu]
&\ul{\gamma}\ar@{-->}[l]\ar[uuu]
&\ul{\gamma}\ar[uuu]
\ar@{-->}[l]
}
\ecen
+
\bcen
\xymatrix@C=1pc@R=1.5pc{
&&
\\
\ar@{<->}[r]
&
&
\\
&\ar@{<->}[r]
&
\\
\ul{\gamma}\ar[uuu]
&\ul{\gamma}\ar@{-->}[l]\ar[uuu]
&\ul{\gamma}\ar[uuu]
\ar@{-->}[l]
}
\ecen
\end{array}
\right]
\label{eq-cala-six-def}
\eeq
Now let us express each of
the 6 birdtracks on the right hand
side of Eq.(\ref{eq-cala-six-def}) in terms of $g$'s instead of swaps.

\beq
\bcen
\xymatrix@C=1pc@R=1.5pc{
&&
\\
\ar@{<->}[r]
&
&
\\
\ul{\gamma}\ar[uu]
&\ul{\gamma}\ar@{-->}[l]\ar[uu]
&\ul{\gamma}\ar[uu]
\ar@{-->}[l]
}
\ecen
=
2
\bcen
\xymatrix@C=1pc@R=1.5pc{
%\ar@{-}`d[ddr]`[r][r]
\ar@{-}@/_1pc/[r]|{\ul{g}}
&
&
\\
&
&
\\
&
&
\ar@{-->}[ll]\ul{\gamma}\ar[uu]
}
\ecen
-
\bcen
\xymatrix@C=1pc@R=1.5pc{
&&
\\
&
&
\\
\ul{\gamma}\ar[uu]
&\ul{\gamma}\ar@{-->}[l]\ar[uu]
&\ul{\gamma}\ar[uu]
\ar@{-->}[l]
}
\ecen
\eeq


\beq
\bcen
\xymatrix@C=1pc@R=1.5pc{
&&
\\
&\ar@{<->}[r]
&
\\
\ul{\gamma}\ar[uu]
&\ul{\gamma}\ar@{-->}[l]\ar[uu]
&\ul{\gamma}\ar[uu]
\ar@{-->}[l]
}
\ecen
=
2
\bcen
\xymatrix@C=1pc@R=1.5pc{
&%\ar@{-}`d[ddr]`[r][r]
\ar@{-}@/_1pc/[r]|{\ul{g}}
&
\\
&
&
\\
\ul{\gamma}\ar[uu]
&
&
\ar@{-->}[ll]
}
\ecen
-
\bcen
\xymatrix@C=1pc@R=1.5pc{
&&
\\
&
&
\\
\ul{\gamma}\ar[uu]
&\ul{\gamma}\ar@{-->}[l]\ar[uu]
&\ul{\gamma}\ar[uu]
\ar@{-->}[l]
}
\ecen
\eeq

\beq
\bcen
\xymatrix@C=1pc@R=1.5pc{
&&
\\
\ar@{<->}[rr]&&
\\
\ul{\gamma}\ar[uu]
&\ul{\gamma}\ar@{-->}[l]\ar[uu]
&\ul{\gamma}\ar[uu]
\ar@{-->}[l]
}
\ecen
=
2
\bcen
\xymatrix@C=1pc@R=1.5pc{
%\ar@{-}`d[ddr]`[r][r]
\ar@{-}@/_1.5pc/[rr]|{\ul{g}}
&
&
\\
&
&
\\
&\ul{\gamma}\ar@{-->}[l]\ar[uu]
&
\ar@{-->}[l]
}
\ecen
-
\bcen
\xymatrix@C=1pc@R=1.5pc{
&&
\\
&
&
\\
\ul{\gamma}\ar[uu]
&\ul{\gamma}\ar@{-->}[l]\ar[uu]
&\ul{\gamma}\ar[uu]
\ar@{-->}[l]
}
\ecen
\eeq


\beqa
\bcen
\xymatrix@C=1pc@R=1.5pc{
&&
\\
&\ar@{<->}[r]
&
\\
\ar@{<->}[r]
&&
\\
\ul{\gamma}\ar[uuu]
&\ul{\gamma}\ar@{-->}[l]\ar[uuu]
&\ul{\gamma}\ar[uuu]
\ar@{-->}[l]
}
\ecen
&=&
2
\bcen
\xymatrix@C=1pc@R=1.5pc{
&
&
\\
&\ar@{<->}[r]
&
\\
\ar[uu]
\ar@{-}@/_1pc/[r]|{\ul{g}}
&\ar[uu]
&
\\
&
&\ul{\gamma}\ar[uuu]
\ar@{-->}[ll]
}
\ecen
-
\bcen
\xymatrix@C=1pc@R=1.5pc{
&&
\\
&\ar@{<->}[r]
&
\\
\ul{\gamma}\ar[uu]
&\ul{\gamma}\ar@{-->}[l]\ar[uu]
&\ul{\gamma}\ar[uu]
\ar@{-->}[l]
}
\ecen
\\
&=&
2
\bcen
\xymatrix@C=1pc@R=1.5pc{
%\ar@{-}`d[ddr]`[r][r]
\ar@{-}@/_1.5pc/[rr]|{\ul{g}}
&
&
\\
&
&
\\
&\ul{\gamma}\ar@{-->}[l]\ar[uu]
&
\ar@{-->}[l]
}
\ecen
-
\bcen
\xymatrix@C=1pc@R=1.5pc{
&&
\\
&\ar@{<->}[r]
&
\\
\ul{\gamma}\ar[uu]
&\ul{\gamma}\ar@{-->}[l]\ar[uu]
&\ul{\gamma}\ar[uu]
\ar@{-->}[l]
}
\ecen
\\
&=&
2
\bcen
\xymatrix@C=1pc@R=1.5pc{
%\ar@{-}`d[ddr]`[r][r]
\ar@{-}@/_1.5pc/[rr]|{\ul{g}}
&
&
\\
&
&
\\
&\ul{\gamma}\ar@{-->}[l]\ar[uu]
&
\ar@{-->}[l]
}
\ecen
-2
\bcen
\xymatrix@C=1pc@R=1.5pc{
&%\ar@{-}`d[ddr]`[r][r]
\ar@{-}@/_1pc/[r]|{\ul{g}}
&
\\
&
&
\\
\ul{\gamma}\ar[uu]
&
&
\ar@{-->}[ll]
}
\ecen
+
\bcen
\xymatrix@C=1pc@R=1.5pc{
&&
\\
&
&
\\
\ul{\gamma}\ar[uu]
&\ul{\gamma}\ar@{-->}[l]\ar[uu]
&\ul{\gamma}\ar[uu]
\ar@{-->}[l]
}
\ecen
\eeqa

\beq
\bcen
\xymatrix@C=1pc@R=1.5pc{
\ar@{<-}[ddd]
&\ar@{<-}[ddd]
&\ar@{<-}[ddd]
\\
\ar@{<->}[r]
&
&
\\
&\ar@{<->}[r]
&
\\
\ul{\gamma}
&\ul{\gamma}\ar@{-->}[l]
&\ul{\gamma}
\ar@{-->}[l]
}
\ecen
=
2
\bcen
\xymatrix@C=1pc@R=1.5pc{
%\ar@{-}`d[ddr]`[r][r]
\ar@{-}@/_1.5pc/[rr]|{\ul{g}}
&
&
\\
&
&
\\
&\ul{\gamma}\ar@{-->}[l]\ar[uu]
&
\ar@{-->}[l]
}
\ecen
-2
\bcen
\xymatrix@C=1pc@R=1.5pc{
%\ar@{-}`d[ddr]`[r][r]
\ar@{-}@/_1pc/[r]|{\ul{g}}
&
&
\\
&
&
\\
&
&
\ar@{-->}[ll]\ul{\gamma}\ar[uu]
}
\ecen
+
\bcen
\xymatrix@C=1pc@R=1.5pc{
&&
\\
&
&
\\
\ul{\gamma}\ar[uu]
&\ul{\gamma}\ar@{-->}[l]\ar[uu]
&\ul{\gamma}\ar[uu]
\ar@{-->}[l]
}
\ecen
\label{eq-arrow-arrow-perm}
\eeq
\qed

\begin{claim}
\beq
\frac{1}{2}
\left[
{\color{red}\gamma_{\nu}}
\gamma_{\mu_1}
\ldots
\gamma_{\mu_a}
-(-1)^a
\gamma_{\mu_1}
\ldots
\gamma_{\mu_a}
{\color{red}\gamma_{\nu}}
\right]
=
\sum_{k=1}^a
(-1)^{k-1}
g_{\nu\mu_k}
\gamma_{\mu_1}
\ldots
\HAT{\gamma_{\mu_k}}
\ldots
\gamma_{\mu_a}
\eeq
where a hat means omission. For $a=2$, 
\beq
\frac{1}{2}
\left[
\bcen
\xymatrix@C=1pc@R=1.5pc{
&&
\\
&
&
\\
\ul{\gamma}\ar@[red][uu]
&\ul{\gamma}\ar@{-->}[l]\ar[uu]
&\ul{\gamma}\ar[uu]
\ar@{-->}[l]
}
\ecen
- (-1)^2
\bcen
\xymatrix@C=1pc@R=1.5pc{
&
&
\\
&
&
\\
\ul{\gamma}\ar[uur]
&\ul{\gamma}\ar@{-->}[l]\ar[uur]
&\ul{\gamma}\ar@[red][uull]
\ar@{-->}[l]
}
\ecen
\right]=
 \bcen
\xymatrix@C=1pc@R=1.5pc{
%\ar@{-}`d[ddr]`[r][r]
\ar@{-}@/_1pc/[r]|{\ul{g}}
&
&
\\
&
&
\\
&
&
\ar@{-->}[ll]\ul{\gamma}\ar[uu]
}
\ecen
-
\bcen
\xymatrix@C=1pc@R=1.5pc{
%\ar@{-}`d[ddr]`[r][r]
\ar@{-}@/_1.5pc/[rr]|{\ul{g}}
&
&
\\
&
&
\\
&\ul{\gamma}\ar@{-->}[l]\ar[uu]
&
\ar@{-->}[l]
}
\ecen
\label{eq-before-after-gamma}
\eeq
\end{claim}
\proof

Note that
\beq
\bcen
\xymatrix@C=1pc@R=1.5pc{
&
&
\\
&
&
\\
\ul{\gamma}\ar[uur]
&\ul{\gamma}\ar@{-->}[l]\ar[uur]
&\ul{\gamma}\ar[uull]
\ar@{-->}[l]
}
\ecen
=
\bcen
\xymatrix@C=1pc@R=1.5pc{
\ar@{<-}[ddd]
&\ar@{<-}[ddd]
&\ar@{<-}[ddd]
\\
\ar@{<->}[r]
&
&
\\
&\ar@{<->}[r]
&
\\
\ul{\gamma}
&\ul{\gamma}\ar@{-->}[l]
&\ul{\gamma}
\ar@{-->}[l]
}
\ecen
\eeq
so this claim has been
proven before for $a=2$ in
Eq.(\ref{eq-arrow-arrow-perm})
\qed

\begin{claim}
If $n\neq a$ and $a$ is odd
\beq
\tr(\gamma_{\mu_1}
\gamma_{\mu_2}
\ldots \gamma_{\mu_a})=0
\eeq
\end{claim}
\proof

If we
left-multiply
both sides of Eq.(\ref{eq-before-after-gamma})
by $\gamma_{\mu_1}$
where $\mu_1$ is the first index,
and then we trace over the spinor indices, we get
\beq
\frac{1}{2}
\left[
\bcen
\xymatrix@C=1pc@R=1.5pc{
&\ar@[red][ldd]
&&
\\
&
&
&
\\
\ul{\gamma}
&\ul{\gamma}\ar@{-->}[l]\ar@[red][uu]
&\ul{\gamma}\ar@{-->}[l]\ar[uu]
&\ul{\gamma}\ar[uu]
\ar@{-->}[l]
\ar@[red]@{-}@/^1.5pc/[lll]
}
\ecen
- (-1)^a
\bcen
\xymatrix@C=1pc@R=1.5pc{
&\ar@[red][ddl]
&
&
\\
&
&
&
\\
\ul{\gamma}
&\ul{\gamma}\ar[uur]\ar@{-->}[l]
&\ul{\gamma}\ar@{-->}[l]\ar[uur]
&\ul{\gamma}\ar@[red][uull]
\ar@{-->}[l]
\ar@[red]@{-}@/^1.5pc/[lll]
}
\ecen
\right]=
 \bcen
\xymatrix@C=1pc@R=1.5pc{
%\ar@{-}`d[ddr]`[r][r]
&
&
&
\\
&
&
&
\\
&\ar@{-->}[l]\ul{\gamma}\ar[uu]
&\ar@{-->}[l]\ul{\gamma}\ar[uu]
&\ar@{-->}[l]
\ar@[red]@{-}@/^1.5pc/[lll]
}
\ecen
-
\bcen
\xymatrix@C=1pc@R=1.5pc{
%\ar@{-}`d[ddr]`[r][r]
&
&
&
\\
&
&
&
\\
&\ul{\gamma}\ar@{-->}[l]\ar[rruu]
&\ul{\gamma}\ar@{-->}[l]\ar[uu]
&\ar@{-->}[l]
\ar@[red]@{-}@/^1.5pc/[lll]
}
\ecen
\eeq
Assuming $a$ is odd, we get

\beq
n
\bcen
\xymatrix@C=1pc{
&&&
\\
\cala_a\ar@2{-}[rrr]
\ar[u]
&\ar[u]
&\ar[u]
&\ar[u]
\\
\ul{\gamma}\ar[u]
&\ul{\gamma}\ar@{-->}[l]\ar[u]
&\ul{\gamma}\ar@{-->}[l]\ar[u]
&\ul{\gamma}\ar@{-->}[l]\ar[u]
\ar@[red]@{-}@/^1.5pc/[lll]
}
\ecen
=
a
\bcen
\xymatrix@C=1pc{
&&&
\\
\cala_a\ar@2{-}[rrr]
\ar[u]
&\ar[u]
&\ar[u]
&\ar[u]
\\
\ul{\gamma}\ar[u]
&\ul{\gamma}\ar@{-->}[l]\ar[u]
&\ul{\gamma}\ar@{-->}[l]\ar[u]
&\ul{\gamma}\ar@{-->}[l]\ar[u]
\ar@[red]@{-}@/^1.5pc/[lll]
}
\ecen
\eeq


%\beq
%\bcen
%\xymatrix@C=1pc@R=1.5pc{
%&
%&
%\\
%&
%&
%\\
%\ul{\gamma}\ar[uur]
%&\ul{\gamma}\ar@{-->}[l]\ar[uur]
%&\ul{\gamma}\ar[uull]
%\ar@{-->}[l]
%}
%\ecen
%=
%\bcen
%\xymatrix@C=1pc@R=1.5pc{
%\ar@{<-}[ddd]
%&\ar@{<-}[ddd]
%&\ar@{<-}[ddd]
%\\
%\ar@{<->}[r]
%&
%&
%\\
%&\ar@{<->}[r]
%&
%\\
%\ul{\gamma}
%&\ul{\gamma}\ar@{-->}[l]
%&\ul{\gamma}
%\ar@{-->}[l]
%}
%\ecen
%=
%2
%\bcen
%\xymatrix@C=1pc@R=1.5pc{
%%\ar@{-}`d[ddr]`[r][r]
%\ar@{-}@/_1.5pc/[rr]|{\ul{g}}
%&
%&
%\\
%&
%&
%\\
%&\ul{\gamma}\ar@{-->}[l]\ar[uu]
%&
%\ar@{-->}[l]
%}
%\ecen
%-2
%\bcen
%\xymatrix@C=1pc@R=1.5pc{
%%\ar@{-}`d[ddr]`[r][r]
%\ar@{-}@/_1pc/[r]|{\ul{g}}
%&
%&
%\\
%&
%&
%\\
%&
%&
%\ar@{-->}[ll]\ul{\gamma}\ar[uu]
%}
%\ecen
%+
%\bcen
%\xymatrix@C=1pc@R=1.5pc{
%&&
%\\
%&
%&
%\\
%\ul{\gamma}\ar[uu]
%&\ul{\gamma}\ar@{-->}[l]\ar[uu]
%&\ul{\gamma}\ar[uu]
%\ar@{-->}[l]
%}
%\ecen
%\eeq
%
%\beqa
%\bcen
%\xymatrix@C=1pc@R=1.5pc{
%&&
%\\
%\ar[u]
%&\cala_2\ar@2{-}[r]\ar[u]
%&\ar[u]
%\\
%&
%&
%\\
%\ul{\gamma}\ar[uur]
%&\ul{\gamma}\ar@{-->}[l]\ar[uur]
%&\ul{\gamma}\ar[uull]
%\ar@{-->}[l]
%}
%\ecen
%&=&
%2
%\bcen
%\xymatrix@C=1pc@R=1.5pc{
%&&
%\\
%%\ar@{-}`d[ddr]`[r][r]
%\ar@{-}@/_1.5pc/[rr]|{\ul{g}}
%\ar[u]
%&\cala_2\ar@2{-}[r]\ar[u]
%&\ar[u]
%\\
%&
%&
%\\
%&\ul{\gamma}\ar@{-->}[l]\ar[uu]
%&
%\ar@{-->}[l]
%}
%\ecen
%-2
%\bcen
%\xymatrix@C=1pc@R=1.5pc{
%&&
%\\
%%\ar@{-}`d[ddr]`[r][r]
%\ar@{-}@/_1pc/[r]|{\ul{g}}
%\ar[u]
%&\cala_2\ar@2{-}[r]\ar[u]
%&\ar[u]
%\\
%&
%&
%\\
%&
%&
%\ar@{-->}[ll]\ul{\gamma}\ar[uu]
%}
%\ecen
%+
%\bcen
%\xymatrix@C=1pc@R=1.5pc{
%&&
%\\
%&\cala_2\ar@2{-}[r]\ar[u]
%&\ar[u]
%\\
%&
%&
%\\
%\ul{\gamma}\ar[uuu]
%&\ul{\gamma}\ar@{-->}[l]\ar[uu]
%&\ul{\gamma}\ar[uu]
%\ar@{-->}[l]
%}
%\ecen
%\\
%&=&
%2 a \indi(a \text{
%odd})
%\bcen
%\xymatrix@C=1pc@R=1.5pc{
%&&
%\\
%%\ar@{-}`d[ddr]`[r][r]
%\ar@{-}@/_1.5pc/[rr]|{\ul{g}}
%\ar[u]
%&\cala_a\ar@2{-}[r]\ar[u]
%&\ar[u]
%\\
%&
%&
%\\
%&\ul{\gamma}\ar@{-->}[l]\ar[uu]
%&
%\ar@{-->}[l]
%}
%\ecen
%+ (-1)^a
%\bcen
%\xymatrix@C=1pc@R=1.5pc{
%&&
%\\
%&\cala_a\ar@2{-}[r]\ar[u]
%&\ar[u]
%\\
%&
%&
%\\
%\ul{\gamma}\ar[uuu]
%&\ul{\gamma}\ar@{-->}[l]\ar[uu]
%&\ul{\gamma}\ar[uu]
%\ar@{-->}[l]
%}
%\ecen
%\eeqa
%
%\beq
%\bcen
%\xymatrix@C=1pc@R=1.5pc{
%\ar[rrrddd]
%&&&
%\\
%\ar[u]
%&\cala_a\ar@2{-}[r]\ar[u]
%&\ar[u]
%&
%\\
%&
%&
%&
%\\
%\ul{\gamma}\ar[uur]
%&\ul{\gamma}\ar@{-->}[l]\ar[uur]
%&\ul{\gamma}\ar[uull]
%\ar@{-->}[l]
%&\ul{\gamma}\ar@{-->}[l]
%\ar@[red]@{-}@/^1.5pc/[lll]
%}
%\ecen
%=
%2 a \indi(a \text{
%odd})
%\bcen
%\xymatrix@C=1pc@R=1.5pc{
%&&
%\\
%%\ar@{-}`d[ddr]`[r][r]
%&\cala_a\ar@2{-}[r]\ar[u]
%&\ar[u]
%\\
%&
%&
%\\
%&\ul{\gamma}\ar@{-->}[l]\ar[uu]
%&\ul{\gamma}\ar@{-->}[l]\ar[uu]
%\ar@[red]@{-}@/^1.5pc/[ll]
%}
%\ecen
%+ (-1)^a
%\bcen
%\xymatrix@C=1pc@R=1.5pc{
%\ar[rrrddd]
%&&&
%\\
%&\cala_a\ar@2{-}[r]\ar[u]
%&\ar[u]
%&
%\\
%&
%&
%&
%\\
%\ul{\gamma}\ar[uuu]
%&\ul{\gamma}\ar@{-->}[l]\ar[uu]
%&\ul{\gamma}\ar[uu]
%\ar@{-->}[l]
%&\ul{\gamma}\ar@{-->}[l]
%\ar@[red]@{-}@/^1.5pc/[lll]
%}
%\ecen
%\eeq
%
%
%\beq
%0=\underbrace{[2a\indi(a \text{
%odd})  + ((-1)^a-1)n]}_{
%\left\{
%\begin{array}{ll}
%2(a-n)&\text{ if $a$ odd}
%\\
%0&\text{ if $a$ even}
%\end{array}
%\right.
%}
%\bcen
%\xymatrix@C=1pc{
%&&&
%\\
%\cala_a\ar@2{-}[rrr]
%\ar[u]
%&\ar[u]
%&\ar[u]
%&\ar[u]
%\\
%\ul{\gamma}\ar[u]
%&\ul{\gamma}\ar@{-->}[l]\ar[u]
%&\ul{\gamma}\ar@{-->}[l]\ar[u]
%&\ul{\gamma}\ar@{-->}[l]\ar[u]
%\ar@[red]@{-}@/^1.5pc/[lll]
%}
%\ecen
%\eeq

Hence, if  $n\neq a$
and $a$ is odd, the trace of $a$ 
gammas is zero.

The above proof is now  complete
and it works for odd or even $n$. However, let us mention that for even $n$,
a chirality operator $\Gamma_5$,  exists,
and this claim  can be proven using $\Gamma_5$. Indeed, for $n$ even, let

\beq
\Gamma_5 =K \gamma_1\gamma_2\ldots 
\gamma_n
\eeq
$\Gamma_5$ anti-commutes with all $\gamma_\mu$:

\beq
\Gamma_5 \gamma_\mu \Gamma_5^{-1}=
-\gamma_\mu
\eeq
Hence

\beqa
\tr(\gamma_{\mu_1}\gamma_{\mu_2}
\ldots\gamma_{\mu_a})
&=&
\tr(\Gamma_5\gamma_{\mu_1}\gamma_{\mu_2}
\ldots\gamma_{\mu_a}
\Gamma_5^{-1})
\\
&=&
(-1)^a\tr(\gamma_{\mu_1}\gamma_{\mu_2}
\ldots\gamma_{\mu_a})
\eeqa
So for odd $a$,
$\tr(\gamma_{\mu_1}\gamma_{\mu_2}
\ldots\gamma_{\mu_a})=0$.

\qed

\begin{claim}
\beq
\begin{array}{l}
\myboxed{
\underbrace{\frac{1}{2}
\tr([\gamma_\mu, \gamma_\nu]_+)}
_{\tr(\gamma_\mu\gamma_\nu)}
=\dashbubble g_{\mu\nu}
}
\\
\underbrace{
\bcen
\xymatrix{
\mu
&\ar[l]
\ar@/^1pc/@{-->}[r]
{\ul{\gamma}}
&\ar@/^1pc/@{-->}[l]
\ul{\gamma}
\ar[r]
&
\nu
}
\ecen
}_{
\bcen
\xymatrix{ 
&\ar@{<-}[d]
&\ar@{<-}[d]
&
\\
&\ul{\gamma}\ar@{-->}[l]
&\ul{\gamma} \ar@{-->}[l]
&\ar@{-->}[l]
\ar@[red]@{-}@/^1pc/[lll]
}
\ecen
}
=
\dashbubble
\xymatrix@C=1pc{
\mu
&\ar[l]\ar[r]\ul{g}
&
\nu
}
\end{array}
\eeq

\beq
\begin{array}{l}
\myboxed{
\tr(\gamma_\mu\gamma_\nu
\gamma_\rho\gamma_\s) =
\dashbubble
(g_{\mu\s} g_{\nu\rho}
-g_{\mu\rho}g_{\nu\s}
+ g_{\mu\nu}g_{\s\rho})
}
\\
\bcen
\xymatrix@C=1pc{ 
&\ar@{<-}[d]\mu
&\ar@{<-}[d]\nu
&\ar@{<-}[d]\rho
&\ar@{<-}[d]\s
&
\\
&\ul{\gamma} \ar@{-->}[l]
&\ul{\gamma} \ar@{-->}[l]
&\ul{\gamma}
\ar@{-->}[l]
&\ul{\gamma} \ar@{-->}[l]
&\ar@{-->}[l]
\ar@[red]@{-}@/^1pc/[lllll]
}
\ecen
=
\dashbubble
\left[
\bcen
\xymatrix@C=1pc{ 
\ar@{-}@/_2pc/[rrr]|{\ul{g}}
&\ar@{-}@/_1pc/[r]|{\ul g}
&
&
}
\ecen
-
\bcen
\xymatrix@C=1pc{ 
\ar@{-}@/_2pc/[rr]|{\ul{g}}
&\ar@{-}@/_1pc/[rr]|{\ul g}
&
&
}
\ecen
+ \bcen
\xymatrix@C=.8pc{ 
\ar@{-}@/_2pc/[r]|{\ul{g}}
&
&\ar@{-}@/_1pc/[r]|{\ul g}
&
}
\ecen
\right]
\end{array}
\eeq
\end{claim}
\proof
\qed

Define the antisymmetrized gamma
matrix products $\Gamma^{(k)}$ by:

\beq
\begin{array}{ccccccc}
\Gamma^{(0)}
&=&
1
&=&
\xymatrix{&\ar@{-->}[l]
}
&=&
\bcen
\xymatrix{
&
&
\\
&\ar@{-->}[l]
\ul{\Gamma}^{(0)}\ar[u]
&\ar@{-->}[l]
}
\ecen
\\
\Gamma^{(1)}_\mu
&=&
\gamma_\mu
&=&
\bcen
\xymatrix{
&
&
\\
&\ar@{-->}[l]
\ul{\gamma}\ar[u]
&\ar@{-->}[l]
}
\ecen
&=&
\bcen
\xymatrix{
&
&
\\
&\ar@{-->}[l]
\ul{\Gamma}^{(1)}\ar[u]
&\ar@{-->}[l]
}
\ecen
\\
\Gamma^{(2)}_{\mu\nu}
&=&
\frac{1}{2}
[\gamma_\mu, \gamma_\nu]
&=&
\bcen
\xymatrix@R=1pc@C=1pc@R=1.5pc{
&&&
\\
&\ar[u]\cala_2 \ar@2{-}[r]
&\ar[u]
&
\\
&\ar@{-->}[l]
\ul{\gamma}\ar[u]
&\ar@{-->}[l]
\ul{\gamma}\ar[u]
&\ar[l]
}
\ecen
&=&
\bcen
\xymatrix{
&
&
\\
&
\ar@{-->}[l]
\ul{\Gamma}^{(2)}\ar[u]
&\ar@{-->}[l]
}
\ecen
\\
\Gamma^{(3)}_{\lam\mu\nu}
&=&
\frac{1}{6}
[\gamma_\lam,\gamma_\mu, \gamma_\nu]
&=&
\bcen
\xymatrix@R=1pc@C=1pc@R=1.5pc{
&&&
\\
&\ar[u]\cala_3 \ar@2{-}[rr]
&\ar[u]
&\ar[u]
&
\\
&\ar@{-->}[l]\ul{\gamma}\ar[u]
&\ar@{-->}[l]\ul{\gamma}\ar[u]
&\ar@{-->}[l]\ul{\gamma}\ar[u]
&\ar@{-->}[l]
}
\ecen
&=&
\bcen
\xymatrix{
&
&
\\
&\ar@{-->}[l]\ul{\Gamma}^{(3)}
\ar[u]
&\ar@{-->}[l]
}
\ecen
\end{array}
\eeq

Henceforth, let
\beq
\ul{g}^{(t)}= \prod_{i=1}^t
g_{\mu_i\nu_i}
\eeq


\begin{claim}
\beq
\underbrace{
\bcen
\xymatrix{
\mu^{:a}
&\ar[l]
\ar@/^1pc/@{-->}[r]
{\ul{\Gamma}^{(a)}}
&\ar@/^1pc/@{-->}[l]
\ul{\Gamma}^{(b)}
\ar[r]
&
\nu^{:b}
}
\ecen
}_{
\bcen
\xymatrix{ 
&
&
&
\\
&\ul{\Gamma}^{(a)}\ar@{-->}[l]\ar[u]
&\ul{\Gamma}^{(b)} \ar@{-->}[l]
\ar[u]
&\ar@{-->}[l]
\ar@[red]@{-}@/^1pc/[lll]
}
\ecen
}
=
\delta_a^b
\dashbubble
\quad
\xymatrix@C=1pc{
\mu^{:a}
&\ar[l]\ar[r]\ul{g}^{(a)}
&\cala_a\ar[r]
&
\nu^{:a}
}
\eeq
\end{claim}
\proof
\qed

Define $\chi_c$ by

\beq
\chi_c=
\bcen
\xymatrix{
&\ar[l]
\cala_b
\ar@{<->}[dr]|{\ul{g}^{(s)}}
\ar@{<->}[rr]|{\ul{g}^{(t)}}
&
&
\ar[r]
\cala_a
&
\\
&
&\cala_c
\ar@{<->}[ur]|{\ul{g}^{(u)}}
\ar[d]
&&
\\
&&&&
}
\ecen
\eeq
where

\beq
\begin{array}{l}
s=(b+c-a)/2
\\
t=(b+a-c)/2
\\
u=(a+c-b)/2
\end{array}
\eeq

\begin{claim}

\beq
\underbrace{
\bcen
\xymatrix@C=1.5pc{
&\ar[l]
\ul{\Gamma}^{(b)}
\ar@{-->}[dr]
&
&\ar@{-->}[ll]
\ar[r]
\ul{\Gamma}^{(a)}
&
\\
&
&\ul{\Gamma}^{(c)}
\ar@{-->}[ur]
\ar[d]
&&
\\
&&&&
}
\ecen}_{
\bcen
\xymatrix@C=1.5pc{ 
&
&
&
\\
&\ul{\Gamma}^{(c)}\ar@{-->}[l]\ar[u]
&\ul{\Gamma}^{(b)}\ar@{-->}[l]\ar[u]
&\ul{\Gamma}^{(a)} \ar@{-->}[l]\ar[u]
&\ar@{-->}[l]
\ar@[red]@{-}@/^1pc/[llll]
}
\ecen
}
=
\frac{a!b!c!}
{s!t!u!}
\dashbubble
\underbrace{
\bcen
\xymatrix{
&\ar[l]
\cala_b
\ar@{<->}[dr]|{\ul{g}^{(s)}}
\ar@{<->}[rr]|{\ul{g}^{(t)}}
&
&
\ar[r]
\cala_a
&
\\
&
&\cala_c
\ar@{<->}[ur]|{\ul{g}^{(u)}}
\ar[d]
&&
\\
&&&&
}
\ecen}_{\chi_c}
\eeq

\end{claim}
\proof
\qed

\begin{claim}
\beq
\bcen
\xymatrix{
&&&
\\
&\ul{\Gamma}^{(b)}\ar@{-->}[l]\ar[u]
&\ul{\Gamma}^{(a)}\ar@{-->}[l]\ar[u]
&\ar@{-->}[l]
}
\ecen
=
\sum_{c=1}^{a+b} K_{c}
\bcen
\xymatrix@C=1.5pc{
&&
\\
\cala_b\ar[u]
&\ar[l]
\ar[r]\ul{g}^{(t)}
&\cala_a\ar[u]
\\
&\ar[ul]|s
\ar[ur]|u
\ul{\Gamma}^{(c)}\ar@{-->}[l]
&\ar@{-->}[l]
}
\ecen
\label{eq-Gamma-expansion}
\eeq
where $t=a-u=b-s$ and 

\beq
K_c =\frac{a!b!c!}{s!t!u!}
\eeq
\end{claim}
\proof

Eq.(\ref{eq-Gamma-expansion}) follows 
because the $\Gamma^{(c)}$
span the vector space of $\Gamma^{(c)}$
products.

If we
left-multiply
both sides of Eq.(\ref{eq-Gamma-expansion})
by $\Gamma^{(c')} $
and then we trace over the spinor indices, we get

\beq
\bcen
\xymatrix{
&&&
\\
&\ul{\Gamma}^{(c')}\ar@{-->}[l]\ar[u]
&\ul{\Gamma}^{(b)}\ar@{-->}[l]\ar[u]
&\ul{\Gamma}^{(a)}\ar@{-->}[l]\ar[u]
&\ar@{-->}[l]\
\ar@[red]@/^1pc/@{-}[llll]
}
\ecen
=
\sum_{c=1}^{a+b} K_{c}
\bcen
\xymatrix@C=1.5pc{
&&&
\\
&\cala_b\ar[u]
&\ar[l]
\ar[r]\ul{g}^{(t)}
&\cala_a\ar[u]
\\
&\ul{\Gamma}^{(c')}\ar@{-->}[l]
\ar[ul]
&\ar[ul]|s
\ar[ur]|u
\ul{\Gamma}^{(c)}\ar@{-->}[l]
&\ar@{-->}[l]
\ar@[red]@/^1pc/@{-}[lll]
}
\ecen
\eeq
so $K_c$ satisfies



\beq
\frac{a!b!c!}
{s!t!u!}
\dashbubble
\chi_c=K_c
\dashbubble \chi_c
\eeq
Hence,

\beq
K_c =\frac{a!b!c!}{s!t!u!}
\eeq
\qed

Define the projector $P^{(a)}$ by
\beq
P^{(a)}=
\frac{1}{\dashbubble }
\bcen
\xymatrix@C=1pc@R=1pc{
\ar@{-->}@/^1pc/[dr]
&&&&
\\
&\ul{\Gamma}^{(a)}
\ar@{-->}@/^1pc/[dl]
&\ol{g}^{(a)}
\ar[l]\ar[r]
&\ul{\Gamma}^{(a)}
\ar@{-->}@/^1pc/[ur]
&
\\
&&&
&\ar@{-->}@/^1pc/[ul]
}
\ecen
=
\frac{1}{\dashbubble}
\bcen
\xymatrix@C=1pc@R=1pc{
\ar@{-->}@/^1pc/[dr]
&&&
\\
&\ul{\Gamma}^{(a)}
\ar@{-->}@/^1pc/[dl]
\ar[r]
&\ol{\Gamma}^{(a)}
\ar@{-->}@/^1pc/[ur]
&
\\
&&
&\ar@{-->}@/^1pc/[ul]
}
\ecen
\eeq
and the 3 leg vertex 
$\stackrel{b\A a}{c}$ by
\beq
\bcen
\xymatrix@C=1.5pc@R=1.5pc{
&&
\\
&\stackrel{b\A a}{c}\ar[ul]
\ar[ur]\ar[d]
&
\\
&&
}
\ecen
=
\frac{1}{\dashbubble}
\bcen
\xymatrix@C=.7pc{
&&&
\\
&\ul{\Gamma}^{(c)}\ar@{-->}[l]\ar[u]
&\ul{\Gamma}^{(b)}\ar@{-->}[l]\ar[u]
&\ul{\Gamma}^{(a)}\ar@{-->}[l]\ar[u]
&\ar@{-->}[l]
\ar@{-}@[red]@/^1pc/[llll]
}
\ecen
=
K_c \chi_c
\eeq
Note that the vertex $\stackrel{b\A a}{c}$
is
nonzero iff $a + b + c$ is even, and if $a, b,$ and $c$ satisfy the triangle inequalities $|a-b| \leq c \leq |a+b|$

\begin{claim}
\beq
\bcen
\xymatrix@C=1.5pc@R=1.5pc{
&&
\\
&\stackrel{a\A b}{c}\ar[ul]
\ar[ur]\ar[d]
&
\\
&&
}
\ecen
=
(-1)^{st+tu+us}
\bcen
\xymatrix@C=1.5pc@R=1.5pc{
&&
\\
&\stackrel{b\A a}{c}\ar[ul]
\ar[ur]\ar[d]
&
\\
&&
}
\ecen
\eeq
\end{claim}
\proof
\qed

Note that

\beqa
d^{(a)}=
\tr(P^{(a)})&=&
\frac{1}{\dashbubble}
\bcen
\xymatrix{
\ul{\Gamma}^{(a)}
\ar@{-->}@/_1pc/[r]
\ar[r]
&
\ol{\Gamma}^{(a)}
\ar@{-->}@/_1pc/[l]
}
\ecen
\\
&=&
\bcen
\xymatrix@C=2pc{
&\ar[l]
\cala_a
&\ar[l]
\ar@/^1pc/@{-}@[red][ll]
}
\ecen
\\
&=&
\left\{
\begin{array}{ll}
{n \choose a}
&\text{if } a\leq n
\text{ (see
 Eq.(\ref{eq-dim-antisym-p}))}
\\
0 & \text{otherwise }
\end{array}
\right.
\eeqa

\beq
\sum_{a=1}^n d^{(a)}=\sum_{a=1}^n{n\choose a}
= (1+1)^2 = 2^a
\eeq

\begin{claim}
\beq
\bcen
\xymatrix{
&&&
\\
&\ul{\Gamma}^{(b)}\ar@{-->}[l]\ar[u]
&\ul{\Gamma}^{(a)}\ar@{-->}[l]\ar[u]
&\ar@{-->}[l]
}
\ecen
=
\sum_{c=1}^{a+b} K'_{c}
\bcen
\xymatrix@C=1.5pc@R=1.5pc{
&&
\\
&\stackrel{b\A a}{c}\ar[ul]
\ar[ur]\ar[d]
&
\\
&\ar@{-->}[l]
\ol{\Gamma}^{(c)}
&\ar@{-->}[l]
}
\ecen
\label{eq-Gamma-expansion-3leg}
\eeq
where

\beq
K_c' =\frac{a!b!c!}{s!t!u!} = K_c
\eeq
\end{claim}
\proof

Eq.(\ref{eq-Gamma-expansion-3leg}) follows 
because the $\Gamma^{(c)}$
span the vector space of $\Gamma^{(c)}$
products.

If we
left-multiply
both sides of Eq.(\ref{eq-Gamma-expansion-3leg})
by $\Gamma^{(c')} $
and then we trace over the spinor indices, we get
\beq
\bcen
\xymatrix{
&&&
\\
&\ul{\Gamma}^{(c')}\ar@{-->}[l]\ar[u]
&\ul{\Gamma}^{(b)}\ar@{-->}[l]\ar[u]
&\ul{\Gamma}^{(a)}\ar@{-->}[l]\ar[u]
&\ar@{-->}[l]\
\ar@[red]@/^1pc/@{-}[llll]
}
\ecen =
\sum_{c=1}^{a+b}
K'_c
\bcen
\xymatrix@C=1.5pc@R=1.5pc{
&&&
\\
&&\stackrel{b\A a}{c}\ar[ul]
\ar[ur]\ar[d]
&
\\
&\ar@{-->}[l]
\ul{\Gamma}^{(c')}\ar[u]
&\ar@{-->}[l]
\ol{\Gamma}^{(c)}
&\ar@{-->}[l]
\ar@[red]@/^1pc/@{-}[lll]
}
\ecen
\eeq
So $K_c'$ satisfies

\beq
\frac{a!b!c!}
{s!t!u!}
\dashbubble
\chi_c=K_c'
\dashbubble \chi_c
\eeq
Hence,
\beq
K_c' =\frac{a!b!c!}{s!t!u!} = K_c
\eeq
\qed

\begin{claim}(t-channel to sum of s-channels)
\beq
\bcen
\xymatrix{
&\ar[d]
\ul{\Gamma}^{(a)}
\ar@{-->}[l]
&\ar@{-->}[l]
\\
\ar@{-->}[r]&\ol{\Gamma}^{(a)}
\ar@{-->}[r]&
}
\ecen
=
\sum_b
\Phi_b
\bcen
\xymatrix@C=1pc@R=1pc{
&&&
\ar@{-->}@/_1pc/[dl]
\\
&\ul{\Gamma}^{(b)}
\ar[r]
\ar@{-->}@/_1pc/[ul]
&\ol{\Gamma}^{(b)}
\ar@{-->}@/_1pc/[dr]
&
\\
\ar@{-->}@/_1pc/[ur]&&
&
}
\ecen
\eeq
where
\newcommand{\sixjspinor}[0]{
\xymatrix@R=2pc@C=2pc{
&\ul{\Gamma}^{(a)}\ar[d]
\ar@/_1pc/@{-->}[ddl]
&
\\
&\ol{\Gamma}^{(a)}
\ar@{-->}[dr]
&
\\
\ol{\Gamma}^{(b)}
\ar@{-->}[ur]
&
&\ul{\Gamma}^{(b)}
\ar@{-->}@/_1pc/[luu]\ar[ll]
}
}

\begin{align}
\Phi_b
&=
\frac{d_b}
{\dashbubble
}
\frac{d_b}{
\dashbubble
}
\frac{
\sixjspinor
}
{d_b}
\\
&=
d_b
\frac{
\sixjspinor
}
{\dashbubble\dashbubble
}
\end{align}


\end{claim}
\proof


\begin{align}
\bcen
\xymatrix{
&\ul{\Gamma}^{(a)}
\ar@{-->}[l]
\ar[d]
&\ar@{-->}[l]
\\
\ar@{-->}[r]
&\ol{\Gamma}^{(a)}
\ar@{-->}[r]
&
}
\ecen
&=
\sum_b
\left[
\begin{array}{l}
\frac{d_b}
{\dashbubble
}
\frac{d_b}
{\dashbubble
}
\\
*
\bcen
\xymatrix@R=1pc@C=1pc{
&
&
&\ul{\Gamma}^{(a)}\ar@{-->}[dl]
\ar[dd]
&
&
&\ar@{-->}[dl]
\\
&\ul{\Gamma}^{(b)}\ar@{-->}[lu]
&\ol{\Gamma}^{(b)}\ar[l]
\ar@{-->}[dr]
&
&\ul{\Gamma}^{(b)}
\ar@{-->}[ul]
&\ol{\Gamma}^{(b)}\ar[l]\ar@{-->}[dr]
&
\\
\ar@{-->}[ur]
&
&
&\ol{\Gamma}^{(a)}\ar@{-->}[ur]
&
&
&
}
\ecen
\end{array}
\right]
\\
&=
\sum_b
\Phi_b
\bcen
\xymatrix{
&&&\ar@{-->}[ld]
\\
&\ul{\Gamma}^{(b)}
\ar@{-->}[lu]
&\ol{\Gamma}^{(b)}
\ar[l]\ar@{-->}[dr]
&
\\
\ar@{-->}[ur]&&&
}
\ecen
\end{align}
\qed

