\chapter{Tensor and Diagrammatic Notation}
\label{ch-tensor-dia-not}
\beqa
P(y) &=&\sum_x P(y|x)P(x)
\\
\av{y|\psi} &=& \sum_x \underbrace{\av{y|A|x}}_{A(y|x)}\av{x|\psi}
\eeqa

\beq
\xymatrix{&\ar[l]}=\xymatrix{&\ar[l]^{\sum a}} =\sum_a \ket{a}\bra{a}
\eeq

\beqa
\av{a|q} &=& \sum_b\av{a|G|b}\av{b|q}
\\
q_a &=&  \sum_b G^b_a q_b
\\
\xymatrix{
&q\ar[l]^a}
&=&
\xymatrix{&G\ar[l]^a & q\ar[l]^{\Sigma b}
}
\eeqa




\beqa
\av{q|a} &=& \sum_b\av{b|G^\dagger|a}\av{q|b}
\\
q^a &=&  \sum_b (G^\dagger)_b^a q^b
\\
\xymatrix{
q&\ar[l]^a}
&=&
\xymatrix{q&G^\dagger\ar[l]^{\sum b}&\ar[l]^a
}
\eeqa

\beq\xymatrix{
&q\ar[l]^a}
=
\xymatrix{a&q\ar[l]}
\eeq

\beq\xymatrix{
q&\ar[l]^a}
=
\xymatrix{
q&a\ar[l]
}\eeq

\beq
G_{a,b,c}^{d,e} = \av{a,b,c|G| d,e} =
\xymatrix{a & G\ar[l]\ar[ld]\ar[ldd] & d\ar[l]
\\
b&&e\ar[lu]
\\
c}
\eeq

\beqa
\av{b_1, b_2|h|a_1, a_2}
&=&
\av{G^\dagger b_1, G^\dagger b_2|h|Ga_1, Ga_2}
\\
\xymatrix{
a_1\ar[dr]
&&a_2\ar[dl]
\\
&h\ar[dl]\ar[dr]
\\
b_1 & & b_2
}
&=&
\xymatrix@R=15pt{
a_1\ar[d]
&&a_2\ar[d]
\\
G \ar[dr]
&& G\ar[dl]
\\
&h\ar[dl]\ar[dr]
\\
G^\dagger \ar[d]
&& G^\dagger \ar[d]
\\
b_1 & & b_2
}
\eeqa

\beqa
G_b^a &=& \delta_b^a + i\sum_j\eps_j
(T_j)_b^a
\\
\xymatrix{&G\ar[l]^b&\ar[l]^a}
&=&
\xymatrix{&\delta\ar[l]^b&\ar[l]^a}
+i\sum_j\eps_j
\xymatrix{&T_j\ar[l]^b&\ar[l]^a}
\eeqa
Assume $T^\dagger_j = T_j$.
To first order in $\eps_j$, 
\beqa
0
 &=& i\sum_j \eps_j
\left(\begin{array}{c}
\xymatrix@R=15pt{
a_1\ar[d]
&&a_2\ar[d]
\\
T_j \ar[dr]
&& \delta\ar[dl]
\\
&h\ar[dl]\ar[dr]
\\
\delta \ar[d]
&& \delta \ar[d]
\\
b_1 & & b_2
}  \xymatrix{\\
\\+}
\xymatrix@R=15pt{
a_1\ar[d]
&&a_2\ar[d]
\\
\delta \ar[dr]
&& T_j\ar[dl]
\\
&h\ar[dl]\ar[dr]
\\
\delta \ar[d]
&&\delta \ar[d]
\\
b_1 & & b_2
}
\end{array}
 \right)
 \\
 &-& i\sum_j \eps_j
\left(\begin{array}{c}
\xymatrix@R=15pt{
a_1\ar[d]
&&a_2\ar[d]
\\
\delta \ar[dr]
&& \delta\ar[dl]
\\
&h\ar[dl]\ar[dr]
\\
T_j \ar[d]
&& \delta \ar[d]
\\
b_1 & & b_2
}  \xymatrix{\\
\\+}
\xymatrix@R=15pt{
a_1\ar[d]
&&a_2\ar[d]
\\
\delta \ar[dr]
&& \delta\ar[dl]
\\
&h\ar[dl]\ar[dr]
\\
\delta \ar[d]
&&T_j \ar[d]
\\
b_1 & & b_2
}
\end{array}
 \right)
\eeqa
from which we get one equation for each $\eps_j$.