\chapter{Lie Algebras}
\label{ch-lie-alg}

$i\in\ZZ_{[1,N]}$, $a,b\in\ZZ_{[1,n]}$

\beq
(C_{Adj}^i)\indices{_b^a}=
\frac{1}{\sqrt{K}}
(T^i)\indices{_b^a}=
\bcen
\xymatrix{
&a\ar[d]
\\
i\ar@{~}[r]
&C_{Adj}^i
\ar[d]
\\
&b
}
\ecen
\eeq
Note that we list the indices of
$T^i$ in the counter-clockwise (CC)
direction, starting at the $i$ leg.
The matrices $T^i$ are called
the generators.
It's customary to choose them so that they are 
Hermitian and $K=\frac{1}{2}$.
\footnote{For $SU(2)$,
it is customary to
use $T^i =\frac{1}{2}\s_i$,
where $\s_i$ for $i=1,2,3$ are the Pauli matrices.
For $SU(3)$,
it is customary to choose $T^i=
\frac{1}{2}\lam_i$
where $\lam_i$
for $i=1,2, \ldots, 8$ are the Gelll-Mann matrices.}

\beq
\begin{array}{ll}
\boxed{
(T^i)\indices{_b^a}(T^j)\indices{_a^b}=
\tr(T^iT^j)=
K \delta(i,j)
}
&
\xymatrix{
i
&T^i\ar@{~}[l]
\ar@/^2pc/[r]|{\sum a}
&T^j
\ar@/^2pc/[l]|{\sum b}
&j\ar@{~}[l]
}
=K
\xymatrix{&\ar[l]|\bullet}
\end{array}
\eeq

\beq
(P_{Adj})_{b,d}^{a,c}
=
\sum_i
\frac{1}{K}
(T^i)\indices{_b^a}
(T^i)\indices{_d^c}
=
\frac{1}{K}
\bcen
\xymatrix@R=1pc@C=1pc{
a\ar[dd]
&
&d
\\
&
&\ar@{~}[ll]
\\
b
&
&c\ar[uu]}
\ecen
\eeq

$H\in V^n\otimes \bar{V}^n$

\beq
(P_{Adj})_{bd}^{ac}H\indices{_c^d}
=
\sum_i (T^i)\indices{_b^a}
\underbrace{
\left[\frac{1}{K}(T^i)\indices{_d^c}
 H\indices{_c^d}
\right]}_{h_i\in\RR}
\eeq

$
G = 1 + i D \in \calg
$

$\eps_i\in\RR $, $|\eps_i|<<1$

$D=\sum_i \eps_i T^i =V^n\otimes \bar{V}^n 
$

Recall Eq.(\ref{eq-xprime-eq-gg-x}).
If $x\in V^{n^p}\otimes \bar{V}^{n^q}$, $\GG\in \calg\subset GL(n^{p+q}, \CC)$,

\beq
(x')\indices{
_{a^{:p}}
^{b^{:q}}
}
=
\GG\indices{
_{a^{:p}}
^{b^{:q}}
_{rev(c^{:q})}
^{rev(d^{:p})}
}
x\indices{
_{d^{:p}}
^{c^{:q}}
},
\quad
(x'_\alp=\GG\indices{_\alp^\beta}x_\beta)
\eeq
where we define

\beq
\GG\indices{
_\alp
^\beta
}
\eqdef
\prod_{i=1}^q
G\indices{
^{b_i}
_{c_i}
}
\prod_{i=1}^p
G\indices{
_{a_i}
^{d_i}
}
\eeq

\beqa
\GG\indices{
_\alp
^\beta}
&=&
 1+i\sum_j\eps_j(\TT^j)
\indices{_\alp^\beta}
\\
G\indices{^{b_i}_{c_i}}
&=&
1+i\sum_j \eps_j 
(T^j)\indices{^{b_i}_{c_i}}
\\
G\indices{_{a_i}^{d_i}}
&=&
(G^*)\indices{^{d_i}_{a_i}}
=
1-i\sum_j\eps_j
(T^{j*})\indices{^{d_i}_{a_i}}
=
1-i\sum_j\eps_j
(T^j)\indices{_{a_i}^{d_i}}
\eeqa

When $x_\alp' =x_\alp$, 
to first order in $\eps_i$,



\beq
0=(\TT^j)\indices{_\alp^\beta}x_\beta=
\left[(T^j)\indices{^{b_i}_{c_i}}
\frac{1}{\delta^{b_i}_{c_i}}
-
(T^j)\indices{_{a_i}^{d_i}}
\frac{1}{\delta_{a_i}^{d_i}}
\right]
\delta
^{b^{:q}}
_{c^{:q}}
\delta
^{d^{:p}}
_{a^{:p}}
x\indices{
_{d^{:p}}
^{c^{:q}}
}
\eeq

\beq
\boxed{
(\TT^j)
\indices{_\alp^\beta}
=
\left[(T^j)\indices{^{b_i}_{c_i}}
\frac{1}{\delta^{b_i}_{c_i}}
-
(T^j)\indices{_{a_i}^{d_i}}
\frac{1}{\delta_{a_i}^{d_i}}
\right]
\delta
^{b^{:q}}
_{c^{:q}}
\delta
^{d^{:p}}
_{a^{:p}}
}
\eeq


