\chapter{Wigner-Ekart Theorem}
\label{ch-wigner-ekart}

\section{WE in general}

\beq
M=
\bcen
\xymatrix@R=1pc{
&M\ar@2{-}[dddddd]
\ar[l]|\mu
\\&
\\
&\ar[l]|\nu
\\&
\\
\ar[r]|\rho&
\\&
\\
\ar[r]|\omega&
}
\ecen
\eeq

\begin{align}
\bcen
\xymatrix@R=1pc{
&M\ar@2{-}[dddddd]
\ar[l]|\mu
\\&
\\
&\ar[l]|\nu
\\&
\\
\ar[r]|\rho&
\\&
\\
\ar[r]|\omega&
}
\ecen
&=
\sum_{\alp, \beta}
\frac{1}{\kappa_\alp \kappa_\beta}
\bcen
\xymatrix@R=1pc{
&\ar[l]&&M
\ar@2{-}[ddddd]
\ar[l]
\\
&T_\alp^\dagger\ar@2{-}[u]
\ar@2{-}[d]&T_\alp\ar@2{-}[u]
\ar@2{-}[d]
\ar[l]
&
\\
&\ar[l]&&\ar[l]
\\
\ar[r]&&\ar[r]&
\\
&T_\beta
\ar@2{-}[u]
\ar@2{-}[d]
\ar[r]
&T_\beta^\dagger\ar@2{-}[u]
\ar@2{-}[d]
&
\\
\ar[r]&&\ar[r]&
}
\ecen
\\
&=
\sum_{\alp}
\frac{1}{\kappa^2_\alp d_\alp}
\bcen
\xymatrix@R=1pc{
&\ar[l]&
\\
&T_\alp^\dagger\ar@2{-}[u]
\ar@2{-}[d]
&
\\
&\ar[l]&
\\
\ar[r]&&
\\
&T_\alp
\ar@2{-}[u]
\ar@2{-}[d]
\ar`r[ruuu]
`[uuu][uuu]
&
\\
\ar[r]&&
}
\xymatrix@R=1pc{
&&M
\ar@2{-}[ddddd]
\ar[l]
\\
&T_\alp\ar@2{-}[u]
\ar@2{-}[d]
\ar`l[ld]
`[ddd][ddd]
&
\\
&&\ar[l]
\\
&\ar[r]&
\\
&T_\alp^\dagger\ar@2{-}[u]
\ar@2{-}[d]
&
\\
&\ar[r]&
}
\ecen
\end{align}


\beq
\bcen
\xymatrix@R=1pc{
&&M
\ar@2{-}[ddddd]
\ar[l]
\\
&T_\alp\ar@2{-}[u]
\ar@2{-}[d]
\ar[l]
&
\\
&&\ar[l]
\\
&\ar[r]&
\\
\ar[r]
&T_\alp^\dagger\ar@2{-}[u]
\ar@2{-}[d]
&
\\
&\ar[r]&
}
\ecen
=\frac{1}{d_\alp}
\bcen
\xymatrix{
&
\\
&
\\
&
\\
\ar
`r[ur]`[uu][uu]&
\\
&
}\ecen
\bcen
\xymatrix@R=1pc{
&&M
\ar@2{-}[ddddd]
\ar[l]
\\
&T_\alp\ar@2{-}[u]
\ar@2{-}[d]
\ar`l[ld]
`[ddd][ddd]
&
\\
&&\ar[l]
\\
&\ar[r]&
\\
&T_\alp^\dagger\ar@2{-}[u]
\ar@2{-}[d]
&
\\
&\ar[r]&
}
\ecen
\eeq




\beq M_a =
\sum_\lam
\xymatrix{
\lam a&\ar[l]
T_\lam
}
\eeq

\beq
M\indices{_\lam_a^\mu^b}=
\xymatrix{
&\ar[l]|\lam
M
&\ar[l]|\mu
}
\eeq

\beq
(M^{\lam i})
\indices{
_{\lam_2 a}
^{\lam_1 b}
}=
\frac{1}{d_\mu}
\bcen
\xymatrix{
M\loopdown{5}{|\mu}
}
\ecen
\quad
\delta(\mu, \lam)
\eeq


\beq
(M^{\lam i})
\indices{
_{\lam_2 a}
^{\lam_1 b}
}=
\bcen
\xymatrix@C=3pc{
&&\ar
`l[dl]|\lam
[dl]
\\
&M^\lam
\ar[l]|{\lam_2}
&
\ar[l]|{\lam_1}
}
\ecen
\eeq

\begin{align}
(M^{\lam })
\indices{
_{\lam_2 }
^{\lam_1 }
}
&=
\sum_{\lam_2}
\frac{d_{\lam_2}}
{
\trij
{\lam}
{\lam_2}
{\lam_1}
}
\bcen
\xymatrix@R=1pc{
&&\ar
`l[dl]|\lam
[ddl]
&&\ar[l]
\\
&&
C_{\lam_2}^\dagger
\ar@2{-}[u]
\ar@2{-}[d]
&\ar[l]
C_{\lam_2}
\ar@2{-}[u]
\ar@2{-}[d]
&
&&
\\
&M^\lam
\ar[l]|{\lam_2}
&
\ar[l]|{\lam_1}
&&\ar[l]
}\ecen
\\
&=
\frac{
\bcen
\xymatrix@R=1pc{
&&\ar
`l[dl]|\lam
[ddl]
&
\\
&&
C_{\lam_2}^\dagger
\ar@2{-}[u]
\ar@2{-}[d]
&
\\
&M^\lam
\ar`l[ld]
`[dr]
`[rr]|{\lam_2}
`[ru]
[ru]
&
\ar[l]|{\lam_1}
&
\\
&&&
}\ecen
}{
\trij
{\lam}
{\lam_2}
{\lam_1}
}
\bcen
\xymatrix@C=3pc{
&&\ar
`l[dl]|\lam
[dl]
\\
&T_{\lam_2}
\ar[l]|{\lam_2}
&
\ar[l]|{\lam_1}
}
\ecen
\end{align}

\section{WE for angular momentum}
$\lam=J$, $\lam_i=J_i$ for $i=1,2$.
We will use Greek letters instead of $J$
so as to keep
convention
of using Greek
letters for rep labels. 

$m, m'= -\lam, \
-\lam+1,\ldots, \lam-1, \lam$. Note
$d_\lam = 2\lam + 1$
 
for $i=1,2$, $m_i= -\lam_i, -\lam_i +1,\ldots, \lam_i-1, \lam_i$.  Note
$d_{\lam_i} = 2\lam_i + 1$ 




\beq
\bcen
\xymatrix@R=1pc{
&
&\ar[l]
\lam_1 m_1
\\
\lam m
&\ar[l]
C_\lam
\ar@2{-}[u]
\ar@2{-}[d]
&
\\
&
&\lam_2 m_2
\ar[l]
\\
}
\ecen
\quad
=\quad
\av{
(\lam_1\lam_2)\lam m|
\lam_1 m_1
\lam_2 m_2
}
\eeq

\beq
\\
\xymatrix{
m
&D^\lam
\ar[l]
&\ar[l]m'
}
\quad =\quad
D^\lam_{m m'}(g)
\eeq


\beq
\begin{array}{l}
\myboxed{
D^{\lam_1}_{m_1 m_1'}(g)
D^{\lam_2}_{m_2 m_2'}(g)=
\sum_{\lam, m, m'}
\av{\lam_1 m_1 \lam_2 m_2|
\lam_1 \lam_2 \lam m}
D^\lam_{m m'}(g)
\av{\lam_1 \lam_2 \lam m'
|
\lam_1 m_1' \lam_2 m_2'}
}
\\
\bcen
\xymatrix@R=1pc{
&D^ {\lam_1}
\ar[l]
&\ar[l]
\\
&D^ {\lam_2}\ar[l]
&\ar[l]
}
\ecen
=
\sum_\lam
\bcen
\xymatrix@R=1pc{
&\ar[l]&&&\ar[l]
\\
&C_\lam^\dagger
\ar@2{-}[u]
\ar@2{-}[d]
&
D^\lam\ar[l]
&C_\lam\ar[l]
\ar@2{-}[u]
\ar@2{-}[d]
&
\\
&\ar[l]&&&\ar[l]
}
\ecen
\end{array}
\eeq

tensor operator $M^\lam_m$

\beq
\av{
\lam_2 m_2 |
M^\lam_m
|
\lam_1 m_1}
=
\bcen
\xymatrix{
&&\ar
`l[dl]
[dl]\lam m
\\
\lam_2 m_2
&M^\lam_m
\ar[l]&
\ar[l]\lam_1 m_1
}
\ecen
\eeq


\beq\begin{array}{l}
\myboxed{
\av{\lam_2 m_2 | M^\lam_m |
\lam_1 m_1}=
\av{(\lam \lam_1 )\lam_2 m_2|\lam m 
\lam_1 m_1
}
q(\lam, \lam_1, \lam_2)
}\\
\bcen
\xymatrix{
&&\ar
`l[dl]
[dl]\lam m
\\
\lam_2 m_2
&M^\lam_m
\ar[l]&
\ar[l]\lam_1 m_1
}
\ecen
=
q(\lam, \lam_1, \lam_2)
\bcen
\xymatrix@R=1pc{
&&\ar[l]|\lam
\\
&C_\lam\ar[l]|{\lam_2}
\ar@2{-}[u]
\ar@2{-}[d]
&
\\
&
&\ar[l]|{\lam_1}
}\ecen
\end{array}
\eeq

\beqa
q(\lam, \lam_1, \lam_2)
&=&
\frac{1}{d_{\lam_2}}
\sum_{m_1, m_2, m}
\av{\lam m \lam_1 m_1|
(\lam \lam_1)
\lam_2 m_2}
\av{
\lam_2 m_2|
M^\lam_m
|
\lam_1 m_1
}
\\
&=&
\frac{1}{d_{\lam_2}}
\bcen
\xymatrix@R=1pc{
&&\ar
`l[dl]|\lam
[ddl]
&
\\
&&
C_{\lam_2}^\dagger
\ar@2{-}[u]
\ar@2{-}[d]
&
\\
&M^\lam_m
\ar`l[ld]
`[dr]
`[rr]|{\lam_2}
`[ru]
[ru]
&
\ar[l]|{\lam_1}
&
\\
&&&
}\ecen
\eeqa